rename files/theories

FOF_Tseitin.thy
@@ -1,198 +1,2025 @@
 theory FOF_Tseitin
-  imports Main FOF_Base FOF_Simplify
+  imports Main FOF_Base
 begin
 
-inductive is_prop :: "('v, 'f, 'p) formula \<Rightarrow> bool" where
-Prop: "is_prop (Pred p [])" |
-And: "is_prop f1 \<Longrightarrow> is_prop f2 \<Longrightarrow> is_prop (And f1 f2)" |
-Or: "is_prop f1 \<Longrightarrow> is_prop f2 \<Longrightarrow> is_prop (Or f1 f2)" |
-Not: "is_prop f \<Longrightarrow> is_prop (Not f)"
+lemma "(x \<longleftrightarrow> \<phi>\<^sub>1) = ((\<not> x \<or> \<phi>\<^sub>1) \<and> (\<not> \<phi>\<^sub>1 \<or> x))"
+  by satx
 
-inductive is_prop_literal :: "('v, 'f, 'p) formula \<Rightarrow> bool" where
-Prop: "is_prop_literal (Pred p [])" |
-NProp: "is_prop_literal (Not (Pred p []))"
+lemma "(x \<longleftrightarrow> \<not> \<phi>\<^sub>1) = ((\<not> x \<or> \<not> \<phi>\<^sub>1) \<and> (\<phi>\<^sub>1 \<or> x))"
+  by satx
 
-inductive is_prop_nnf :: "('v, 'f, 'p) formula \<Rightarrow> bool" where
-Prop: "is_prop_nnf (Pred p [])" |
-NProp: "is_prop_nnf (Not (Pred p []))" |
-And: "is_prop_nnf f1 \<Longrightarrow> is_prop_nnf f2 \<Longrightarrow> is_prop_nnf (And f1 f2)" |
-Or: "is_prop_nnf f1 \<Longrightarrow> is_prop_nnf f2 \<Longrightarrow> is_prop_nnf (Or f1 f2)"
+lemma "(x \<longleftrightarrow> \<phi>\<^sub>1 \<and> \<phi>\<^sub>2) = ((\<not> x \<or> \<phi>\<^sub>1) \<and> (\<not> x \<or> \<phi>\<^sub>2) \<and> (\<not> \<phi>\<^sub>1 \<or> \<not> \<phi>\<^sub>2 \<or> x))"
+  by satx
 
-inductive is_prop_clause :: "('v, 'f, 'p) formula \<Rightarrow> bool" where
-Literal: "is_prop_literal f \<Longrightarrow> is_prop_clause f" |
-Or: "is_prop_literal f1 \<Longrightarrow> is_prop_literal f2 \<Longrightarrow> is_prop_clause (Or f1 f2)"
+lemma "(x \<longleftrightarrow> \<phi>\<^sub>1 \<or> \<phi>\<^sub>2) = ((\<not> x \<or> \<phi>\<^sub>1 \<or> \<phi>\<^sub>2) \<and> (\<not> \<phi>\<^sub>1 \<or> x) \<and> (\<not> \<phi>\<^sub>2 \<or> x))"
+  by satx
 
-inductive is_cnf :: "('v, 'f, 'p) formula \<Rightarrow> bool" where
-Literal: "is_prop_literal f \<Longrightarrow> is_cnf f" |
-And: "is_prop_clause f1 \<Longrightarrow> is_prop_clause f2 \<Longrightarrow> is_cnf (And f1 f2)" 
+datatype 'a literal = Pos (atom: 'a) | Neg (atom: 'a)
 
-type_synonym 'p fresh = "'p set \<Rightarrow> 'p"
-type_synonym ('v, 'f, 'p) tseitin_asgnm = "'p \<times> ('v, 'f, 'p) formula"
+type_synonym 'a clause = "'a literal list"
 
-fun tseitin_occup_var :: "('v, 'f, 'p) formula \<Rightarrow> 'p set" where
-"tseitin_occup_var (Pred p []) = {p}" |
-"tseitin_occup_var (Not (Pred p [])) = {p}" |
-"tseitin_occup_var (And f1 f2) = tseitin_occup_var f1 \<union> tseitin_occup_var f2" |
-"tseitin_occup_var (Or f1 f2) = tseitin_occup_var f1 \<union> tseitin_occup_var f2" |
-"tseitin_occup_var _ = {}"
+fun tseitin ::
+  "('p set \<Rightarrow> 'p) \<Rightarrow> 'p set \<Rightarrow> ('v, 'f, 'p) formula \<Rightarrow>
+    'p \<times> ('v, 'f) fof_term list \<times> ('p \<times> ('v, 'f) fof_term list) literal list list \<times> 'p set" where
+  \<comment> \<open>The arguments are
+    a function \<^term>\<open>fresh :: 'p set \<Rightarrow> 'p\<close> to generate fresh variables,
+    a finite set \<^term>\<open>\<V> :: 'p set\<close> of variable not to use, and
+    a formula \<^term>\<open>\<phi> :: ('v, 'f, 'p) formula\<close> to expand.\<close>
+  \<comment> \<open>The result is a 4-tuple \<^term>\<open>((v, ts, \<C>, \<V>'))\<close>, where
+    \<^term>\<open>v :: 'p\<close> is the variable representing the formula,
+    \<^term>\<open>ts :: ('v, 'f) fof_term list\<close> are the arguments to the variable representing the formula,
+    \<^term>\<open>\<C> :: ('p \<times> ('v, 'f) fof_term list) clause list\<close> is the clause list specifying the formula, and
+    \<^term>\<open>\<V>' :: 'p set\<close> is the finite set of fresh variables generated for this formula.\<close>
+  "tseitin fresh \<V> (Pred p ts) = (p, ts, [], {})" |
+  "tseitin fresh \<V> (Not \<phi>\<^sub>1) =
+    (let
+      (v\<^sub>1, ts\<^sub>1, \<C>\<^sub>1, \<V>\<^sub>1) = tseitin fresh \<V> \<phi>\<^sub>1;
+      v = fresh (\<V> \<union> \<V>\<^sub>1);
+      C\<^sub>1 = [Neg (v, []), Neg (v\<^sub>1, ts\<^sub>1)];
+      C\<^sub>2 = [Pos (v, []), Pos (v\<^sub>1, ts\<^sub>1)]
+     in (v, [], C\<^sub>1 # C\<^sub>2 # \<C>\<^sub>1, insert v \<V>\<^sub>1))" |
+  "tseitin fresh \<V> (And \<phi>\<^sub>1 \<phi>\<^sub>2) = 
+    (let
+      (v\<^sub>1, ts\<^sub>1, \<C>\<^sub>1, \<V>\<^sub>1) = tseitin fresh \<V> \<phi>\<^sub>1;
+      (v\<^sub>2, ts\<^sub>2, \<C>\<^sub>2, \<V>\<^sub>2) = tseitin fresh (\<V> \<union> \<V>\<^sub>1) \<phi>\<^sub>2;
+      v = fresh (\<V> \<union> \<V>\<^sub>1 \<union> \<V>\<^sub>2);
+      C\<^sub>1 = [Neg (v, []), Pos (v\<^sub>1, ts\<^sub>1)];
+      C\<^sub>2 = [Neg (v, []), Pos (v\<^sub>2, ts\<^sub>2)];
+      C\<^sub>3 = [Pos (v, []), Neg (v\<^sub>1, ts\<^sub>1), Neg (v\<^sub>2, ts\<^sub>2)]
+     in (v, [], C\<^sub>1 # C\<^sub>2 # C\<^sub>3 # \<C>\<^sub>1 @ \<C>\<^sub>2, insert v (\<V>\<^sub>1 \<union> \<V>\<^sub>2)))" |
+  "tseitin fresh \<V> (Or \<phi>\<^sub>1 \<phi>\<^sub>2) =
+    (let
+      (v\<^sub>1, ts\<^sub>1, \<C>\<^sub>1, \<V>\<^sub>1) = tseitin fresh \<V> \<phi>\<^sub>1;
+      (v\<^sub>2, ts\<^sub>2, \<C>\<^sub>2, \<V>\<^sub>2) = tseitin fresh (\<V> \<union> \<V>\<^sub>1) \<phi>\<^sub>2;
+      v = fresh (\<V> \<union> \<V>\<^sub>1 \<union> \<V>\<^sub>2);
+      C\<^sub>1 = [Pos (v, []), Neg (v\<^sub>1, ts\<^sub>1)];
+      C\<^sub>2 = [Pos (v, []), Neg (v\<^sub>2, ts\<^sub>2)];
+      C\<^sub>3 = [Neg (v, []), Pos (v\<^sub>2, ts\<^sub>2), Pos (v\<^sub>1, ts\<^sub>1)]
+     in (v, [], C\<^sub>1 # C\<^sub>2 # C\<^sub>3 # \<C>\<^sub>1 @ \<C>\<^sub>2, insert v (\<V>\<^sub>1 \<union> \<V>\<^sub>2)))"
 
-fun tseitin_list :: "('v, 'f, 'p) formula \<Rightarrow> ('v, 'f, 'p) formula list" where
-"tseitin_list (Pred p []) = []" |
-"tseitin_list (Not (Pred p [])) = [Not (Pred p [])]" |
-"tseitin_list (And f1 f2) = [And f1 f2] @ tseitin_list f1 @ tseitin_list f2" |
-"tseitin_list (Or f1 f2) = [Or f1 f2] @ tseitin_list f1 @ tseitin_list f2" |
-"tseitin_list _ = []"
+inductive is_nnf where
+  PosPred: "is_nnf (Pred p ts)" |
+  NegPred: "is_nnf (Not (Pred p ts))" |
+  And: "is_nnf \<phi>\<^sub>1 \<Longrightarrow> is_nnf \<phi>\<^sub>2 \<Longrightarrow> is_nnf (And \<phi>\<^sub>1 \<phi>\<^sub>2)" |
+  Or: "is_nnf \<phi>\<^sub>1 \<Longrightarrow> is_nnf \<phi>\<^sub>2 \<Longrightarrow> is_nnf (Or \<phi>\<^sub>1 \<phi>\<^sub>2)"
 
-definition tseitin_fresh_var :: "'p fresh \<Rightarrow> 'p set \<Rightarrow> 'p \<times> 'p set" where
-"tseitin_fresh_var \<xi> \<Sigma> = (let \<tau> = \<xi> \<Sigma> in (\<tau>, \<Sigma> \<union> {\<tau>}))"
+lemma predicates_of_formula_finite: 
+  "finite (predicates_of_formula \<phi>)"
+proof (induction \<phi>)
+  case (Pred p args)
+  then show ?case
+    by simp
+next
+  case (And \<phi>1 \<phi>2)
+  then show ?case
+    by simp
+next
+  case (Or \<phi>1 \<phi>2)
+  then show ?case
+    by simp
+next
+  case (Not \<phi>)
+  then show ?case
+    by simp
+next
+  case (Equal t1 t2)
+  then show ?case
+    by simp
+next
+  case (Forall v1 \<phi>)
+  then show ?case
+    by simp
+next
+  case (Exists v1 \<phi>)
+  then show ?case
+    by simp
+next
+  case T
+  then show ?case
+    by simp
+next
+  case F
+  then show ?case
+    by simp
+qed
 
-fun tseitin_list_asgnm :: 
-"'p fresh \<Rightarrow> 'p set \<Rightarrow> ('v, 'f, 'p) formula list \<Rightarrow> ('v, 'f, 'p) tseitin_asgnm list" where
-"tseitin_list_asgnm \<xi> \<Sigma> [] = []" |
-"tseitin_list_asgnm \<xi> \<Sigma> (f # fs) = 
-  (let fresh_var = tseitin_fresh_var \<xi> \<Sigma>;
-       assign_var = ((fst fresh_var), f)
-    in assign_var # tseitin_list_asgnm \<xi> (snd fresh_var) fs)"
+lemma tseitin_finite_var_set:
+  assumes "is_nnf \<phi>"
+  assumes tseitin: "tseitin fresh \<V> \<phi> = (v, ts, \<C>, \<V>')"
+  shows "finite \<V>'"
+  using assms
+proof (induction \<phi> arbitrary: \<V> v ts \<C> \<V>' rule: is_nnf.induct)
+  case (PosPred p ts)
 
-fun tseitin_subst_formula ::
-"('v, 'f, 'p) formula \<Rightarrow> ('v, 'f, 'p) tseitin_asgnm list \<Rightarrow> ('v, 'f, 'p) formula" where
-"tseitin_subst_formula f [] = f" |
-"tseitin_subst_formula f (a # as) = 
-  (if (f = snd a) 
-   then Pred (fst a) []
-   else tseitin_subst_formula f as)"
+  have "\<V>' = {}"
+    using tseitin local.PosPred 
+    by auto
 
-fun tseitin_subst_subformula :: 
-"('v, 'f, 'p) formula \<Rightarrow> ('v, 'f, 'p) tseitin_asgnm list \<Rightarrow> ('v, 'f, 'p) formula" where
-"tseitin_subst_subformula f [] = f" |
-"tseitin_subst_subformula (Pred p []) _ = Pred p []" |
-"tseitin_subst_subformula (Not (Pred p [])) _ = Not (Pred p [])" |
-"tseitin_subst_subformula (And f1 f2) as = 
-  (let f1_subst = tseitin_subst_formula f1 as;
-       f2_subst = tseitin_subst_formula f2 as
-    in And f1_subst f2_subst)" |
-"tseitin_subst_subformula (Or f1 f2) as =
-  (let f1_subst = tseitin_subst_formula f1 as;
-       f2_subst = tseitin_subst_formula f2 as
-    in Or f1_subst f2_subst)" |
-"tseitin_subst_subformula f _ = f"
+  show ?case
+    by (simp add: \<open>\<V>' = {}\<close>)
+next
+  case (NegPred p ts)
 
-fun tseitin_list_subst :: "('v, 'f, 'p) tseitin_asgnm list \<Rightarrow> ('v, 'f, 'p) tseitin_asgnm list" where
-"tseitin_list_subst [] = []" |
-"tseitin_list_subst ((\<tau>, f) # as) =
-  (let f' = tseitin_subst_subformula f as
-    in (\<tau>, f') # tseitin_list_subst as)"
+  have "v = fresh \<V>" and
+       "\<V>' = insert v {}"
+    unfolding atomize_conj
+    using NegPred.prems[simplified]
+    by (metis prod.inject)
 
+  show ?case
+    by (simp add: \<open>\<V>' = {v}\<close>)
+next
+  case (And \<phi>\<^sub>1 \<phi>\<^sub>2)
+
+  obtain v\<^sub>1 ts\<^sub>1 \<C>\<^sub>1 \<V>\<^sub>1 where
+    te_\<phi>1: "tseitin fresh \<V> \<phi>\<^sub>1 = (v\<^sub>1, ts\<^sub>1, \<C>\<^sub>1, \<V>\<^sub>1)"
+    using prod_cases4 
+    by blast
+
+  obtain v\<^sub>2 ts\<^sub>2 \<C>\<^sub>2 \<V>\<^sub>2 where
+    te_\<phi>2: "tseitin fresh (\<V> \<union> \<V>\<^sub>1) \<phi>\<^sub>2 = (v\<^sub>2, ts\<^sub>2, \<C>\<^sub>2, \<V>\<^sub>2)"
+    using prod_cases4 
+    by blast
+
+  have
+    "v = fresh (\<V> \<union> \<V>\<^sub>1 \<union> \<V>\<^sub>2)" and
+    "\<V>' = insert v (\<V>\<^sub>1 \<union> \<V>\<^sub>2)"
+    unfolding atomize_conj
+    using And.prems[simplified, unfolded te_\<phi>1, simplified, unfolded te_\<phi>2, simplified]
+    by (metis Pair_inject)
+
+  have "finite \<V>\<^sub>1"
+    using And.IH(1) te_\<phi>1 
+    by auto
+
+  have "finite \<V>\<^sub>2"
+    using And.IH(2) te_\<phi>2 
+    by blast
+
+  show ?case
+    by (simp add: \<open>\<V>' = insert v (\<V>\<^sub>1 \<union> \<V>\<^sub>2)\<close> \<open>finite \<V>\<^sub>1\<close> \<open>finite \<V>\<^sub>2\<close>)
+next
+  case (Or \<phi>\<^sub>1 \<phi>\<^sub>2)
+
+  obtain v\<^sub>1 ts\<^sub>1 \<C>\<^sub>1 \<V>\<^sub>1 where
+    te_\<phi>1: "tseitin fresh \<V> \<phi>\<^sub>1 = (v\<^sub>1, ts\<^sub>1, \<C>\<^sub>1, \<V>\<^sub>1)"
+    using prod_cases4 
+    by blast
+
+  obtain v\<^sub>2 ts\<^sub>2 \<C>\<^sub>2 \<V>\<^sub>2 where
+    te_\<phi>2: "tseitin fresh (\<V> \<union> \<V>\<^sub>1) \<phi>\<^sub>2 = (v\<^sub>2, ts\<^sub>2, \<C>\<^sub>2, \<V>\<^sub>2)"
+    using prod_cases4 
+    by blast
+
+  have
+    "v = fresh (\<V> \<union> \<V>\<^sub>1 \<union> \<V>\<^sub>2)" and
+    "\<V>' = insert v (\<V>\<^sub>1 \<union> \<V>\<^sub>2)"
+    unfolding atomize_conj
+    using Or.prems[simplified, unfolded te_\<phi>1, simplified, unfolded te_\<phi>2, simplified]
+    by (metis Pair_inject) 
+
+  have "finite \<V>\<^sub>1"
+    using Or.IH(1) te_\<phi>1
+    by auto
+
+  have "finite \<V>\<^sub>2"
+    using Or.IH(2) te_\<phi>2
+    by auto
+
+  show ?case
+    by (simp add: \<open>\<V>' = insert v (\<V>\<^sub>1 \<union> \<V>\<^sub>2)\<close> \<open>finite \<V>\<^sub>1\<close> \<open>finite \<V>\<^sub>2\<close>)
+qed
+
+lemma tseitin_fresh_vars:
+  fixes fresh :: "'p set \<Rightarrow> 'p"
+  assumes fresh_spec: "\<And>\<V>. finite \<V> \<Longrightarrow> fresh \<V> \<notin> \<V>"
+  assumes "is_nnf \<phi>"
+  assumes "finite \<V>"
+  assumes tseitin: "tseitin fresh \<V> \<phi> = (v, ts, \<C>, \<V>')"
+  shows "\<V> \<inter> \<V>' = {}"
+  using \<open>is_nnf \<phi>\<close> assms
+proof (induction \<phi> arbitrary: \<V> v ts \<C> \<V>' rule: is_nnf.induct)
+  case (PosPred p ts)
+
+  have "\<V>' = {}"
+    using tseitin PosPred.prems(4) 
+    by auto
+
+  show ?case
+    by (simp add: \<open>\<V>' = {}\<close>)
+next
+  case (NegPred p ts)
+
+  have "v = fresh \<V>" and
+       "\<V>' = insert v {}"
+    unfolding atomize_conj
+    using NegPred.prems[simplified]
+    by (metis Pair_inject)
+
+  have "v \<notin> \<V>"
+    using \<open>v = fresh \<V>\<close> fresh_spec
+    by (simp add: NegPred.prems(3))
+
+  show ?case
+    by (simp add: \<open>\<V>' = {v}\<close> \<open>v \<notin> \<V>\<close>)
+next
+  case (And \<phi>\<^sub>1 \<phi>\<^sub>2)
+
+  obtain v\<^sub>1 ts\<^sub>1 \<C>\<^sub>1 \<V>\<^sub>1 where
+    te_\<phi>1: "tseitin fresh \<V> \<phi>\<^sub>1 = (v\<^sub>1, ts\<^sub>1, \<C>\<^sub>1, \<V>\<^sub>1)"
+    using prod_cases4 
+    by blast
+
+  obtain v\<^sub>2 ts\<^sub>2 \<C>\<^sub>2 \<V>\<^sub>2 where
+    te_\<phi>2: "tseitin fresh (\<V> \<union> \<V>\<^sub>1) \<phi>\<^sub>2 = (v\<^sub>2, ts\<^sub>2, \<C>\<^sub>2, \<V>\<^sub>2)"
+    using prod_cases4 
+    by blast
+
+  have
+    "v = fresh (\<V> \<union> \<V>\<^sub>1 \<union> \<V>\<^sub>2)" and
+    "\<V>' = insert v (\<V>\<^sub>1 \<union> \<V>\<^sub>2)"
+    unfolding atomize_conj
+    using And.prems[simplified, unfolded te_\<phi>1, simplified, unfolded te_\<phi>2, simplified]
+    by (metis Pair_inject)
+
+  have "v \<notin> \<V>"
+    using \<open>v = fresh (\<V> \<union> \<V>\<^sub>1 \<union> \<V>\<^sub>2)\<close> fresh_spec
+    by (metis And.hyps(1,2) And.prems(3) Un_iff
+        finite_Un te_\<phi>1 te_\<phi>2 tseitin_finite_var_set)
+
+  have IH1: "\<V> \<inter> \<V>\<^sub>1 = {}" 
+    using And.IH(1) te_\<phi>1
+    by (simp add: And.hyps(1) And.prems(3) fresh_spec)
+
+  have IH2: "(\<V> \<union> \<V>\<^sub>1) \<inter> \<V>\<^sub>2 = {}"
+    using And.IH(2) te_\<phi>2
+    by (metis And.hyps(1,2) And.prems(3)
+        finite_Un fresh_spec te_\<phi>1
+        tseitin_finite_var_set)
+
+  show ?case
+    using IH1 IH2 \<open>\<V>' = insert v (\<V>\<^sub>1 \<union> \<V>\<^sub>2)\<close> \<open>v \<notin> \<V>\<close>
+    by auto
+next
+  case (Or \<phi>\<^sub>1 \<phi>\<^sub>2)
+
+  obtain v\<^sub>1 ts\<^sub>1 \<C>\<^sub>1 \<V>\<^sub>1 where
+    te_\<phi>1: "tseitin fresh \<V> \<phi>\<^sub>1 = (v\<^sub>1, ts\<^sub>1, \<C>\<^sub>1, \<V>\<^sub>1)"
+    using prod_cases4 
+    by blast
+
+  obtain v\<^sub>2 ts\<^sub>2 \<C>\<^sub>2 \<V>\<^sub>2 where
+    te_\<phi>2: "tseitin fresh (\<V> \<union> \<V>\<^sub>1) \<phi>\<^sub>2 = (v\<^sub>2, ts\<^sub>2, \<C>\<^sub>2, \<V>\<^sub>2)"
+    using prod_cases4 
+    by blast
+
+  have
+    "v = fresh (\<V> \<union> \<V>\<^sub>1 \<union> \<V>\<^sub>2)" and
+    "\<V>' = insert v (\<V>\<^sub>1 \<union> \<V>\<^sub>2)"
+    unfolding atomize_conj
+    using Or.prems[simplified, unfolded te_\<phi>1, simplified, unfolded te_\<phi>2, simplified]
+    by (metis Pair_inject)
+
+  have "v \<notin> \<V>"
+    using \<open>v = fresh (\<V> \<union> \<V>\<^sub>1 \<union> \<V>\<^sub>2)\<close> fresh_spec
+    by (metis Or.hyps(1,2) Or.prems(3) Un_iff
+        finite_Un te_\<phi>1 te_\<phi>2 tseitin_finite_var_set)
+
+  have IH1: "\<V> \<inter> \<V>\<^sub>1 = {}" 
+    using Or.IH(1) te_\<phi>1
+    by (simp add: Or.hyps(1) Or.prems(3) fresh_spec)
+
+  have IH2: "(\<V> \<union> \<V>\<^sub>1) \<inter> \<V>\<^sub>2 = {}"
+    using Or.IH(2) te_\<phi>2
+    by (metis Or.hyps(1,2) Or.prems(3) finite_Un
+        fresh_spec te_\<phi>1 tseitin_finite_var_set)
+
+  show ?case
+    using IH1 IH2 \<open>\<V>' = insert v (\<V>\<^sub>1 \<union> \<V>\<^sub>2)\<close> \<open>v \<notin> \<V>\<close>
+    by auto
+qed
+
+lemma
+  fixes \<phi> :: "('v, 'f, 'p) formula"
+  assumes "is_nnf \<phi>"
+  assumes tseitin: "tseitin fresh \<V> \<phi> = (v, ts, \<C>, \<V>')"
+  shows
+    tseitin_generated_var: "v \<in> predicates_of_formula \<phi> \<union> \<V>'" and
+    tseitin_generated_vars: "insert v (\<Union>C \<in> set \<C>. fst ` atom ` set C) = predicates_of_formula \<phi> \<union> \<V>'"
+  unfolding atomize_conj
+  using assms
+proof (induction \<phi> arbitrary: \<V> v ts \<C> \<V>' rule: "is_nnf.induct")
+  case (PosPred p ts\<^sub>p)
+
+  have "v = p" and
+       "\<C> = []" and
+       "\<V>' = {}"
+    unfolding atomize_conj
+    using PosPred.prems[simplified]
+    by simp
+
+  have gen_var: 
+      "v \<in> predicates_of_formula (Pred p ts\<^sub>p) \<union> \<V>'"
+    by (simp add: \<open>v = p\<close>)
+
+  have gen_vars: 
+      "insert v (\<Union>C \<in> set \<C>. fst ` atom ` set C) = predicates_of_formula (Pred p ts\<^sub>p) \<union> \<V>'"
+    unfolding \<open>\<C> = []\<close> \<open>\<V>' = {}\<close>
+    by (simp add: \<open>v = p\<close>)
+
+  show ?case
+    using gen_var gen_vars
+    by simp
+next
+  case (NegPred p ts\<^sub>p)
+
+  define \<C>\<^sub>0 :: "('p \<times> ('v, 'f) fof_term list) literal list list" where
+    "\<C>\<^sub>0 = [
+      [Neg (v, []), Neg (p, ts\<^sub>p)],
+      [Pos (v, []), Pos (p, ts\<^sub>p)]]"
+
+  have "v = fresh \<V>" and
+       "\<C> = \<C>\<^sub>0" and
+       "\<V>' = insert v {}"
+    unfolding atomize_conj
+    using NegPred.prems[simplified]
+    by (metis Pair_inject \<C>\<^sub>0_def)
+
+  have gen_var: 
+      "v \<in> predicates_of_formula (Not (Pred p ts\<^sub>p)) \<union> \<V>'"
+    by (simp add: \<open>\<V>' = {v}\<close>)
+
+  have gen_vars: 
+      "insert v (\<Union>C \<in> set \<C>. fst ` atom ` set C) = predicates_of_formula (Not (Pred p ts\<^sub>p)) \<union> \<V>'"
+    unfolding \<open>\<C> = \<C>\<^sub>0\<close> \<C>\<^sub>0_def \<open>\<V>' = insert v {}\<close>
+    by simp
+
+  show ?case 
+    using gen_var gen_vars
+    by simp
+next
+  case (And \<phi>\<^sub>1 \<phi>\<^sub>2)
+
+  obtain v\<^sub>1 ts\<^sub>1 \<C>\<^sub>1 \<V>\<^sub>1 where
+    te_\<phi>1: "tseitin fresh \<V> \<phi>\<^sub>1 = (v\<^sub>1, ts\<^sub>1, \<C>\<^sub>1, \<V>\<^sub>1)"
+    using prod_cases4 by blast
+
+  obtain v\<^sub>2 ts\<^sub>2 \<C>\<^sub>2 \<V>\<^sub>2 where
+    te_\<phi>2: "tseitin fresh (\<V> \<union> \<V>\<^sub>1) \<phi>\<^sub>2 = (v\<^sub>2, ts\<^sub>2, \<C>\<^sub>2, \<V>\<^sub>2)"
+    using prod_cases4 by blast
+
+  define \<C>\<^sub>0 :: "('p \<times> ('v, 'f) fof_term list) literal list list" where
+    "\<C>\<^sub>0 = [
+      [Neg (v, []), Pos (v\<^sub>1, ts\<^sub>1)], 
+      [Neg (v, []), Pos (v\<^sub>2, ts\<^sub>2)], 
+      [Pos (v, []), Neg (v\<^sub>1, ts\<^sub>1), Neg (v\<^sub>2, ts\<^sub>2)]]"
+
+  have
+    "v = fresh (\<V> \<union> \<V>\<^sub>1 \<union> \<V>\<^sub>2)" and
+    "\<C> = \<C>\<^sub>0 @ \<C>\<^sub>1 @ \<C>\<^sub>2" and
+    "\<V>' = insert v (\<V>\<^sub>1 \<union> \<V>\<^sub>2)"
+    using And.prems[simplified, unfolded te_\<phi>1, simplified, unfolded te_\<phi>2, simplified] 
+    by (auto simp add: \<C>\<^sub>0_def Let_def)
+
+  have gen_var: 
+      "v \<in> predicates_of_formula (And \<phi>\<^sub>1 \<phi>\<^sub>2) \<union> \<V>'"
+    by (simp add: \<open>\<V>' = insert v (\<V>\<^sub>1 \<union> \<V>\<^sub>2)\<close>)
+
+  have gen_vars_\<phi>1: 
+      "insert v\<^sub>1 (\<Union>C \<in> set \<C>\<^sub>1. fst ` atom ` set C) = predicates_of_formula \<phi>\<^sub>1 \<union> \<V>\<^sub>1"
+    using And.IH(1)[OF te_\<phi>1]
+    by simp
+
+  have gen_vars_\<phi>2: 
+      "insert v\<^sub>2 (\<Union>C \<in> set \<C>\<^sub>2. fst ` atom ` set C) = predicates_of_formula \<phi>\<^sub>2 \<union> \<V>\<^sub>2"
+    using And.IH(2)[OF te_\<phi>2]
+    by simp
+
+  have gen_vars: 
+      "insert v (\<Union>C \<in> set \<C>. fst ` atom ` set C) = predicates_of_formula (And \<phi>\<^sub>1 \<phi>\<^sub>2) \<union> \<V>'"
+    unfolding \<open>\<C> = \<C>\<^sub>0 @ \<C>\<^sub>1 @ \<C>\<^sub>2\<close> \<C>\<^sub>0_def \<open>\<V>' = insert v (\<V>\<^sub>1 \<union> \<V>\<^sub>2)\<close>
+    using gen_vars_\<phi>1 gen_vars_\<phi>2
+    by fastforce
+
+  show ?case
+    using gen_var gen_vars
+    by simp
+next
+  case (Or \<phi>\<^sub>1 \<phi>\<^sub>2)
+
+  obtain v\<^sub>1 ts\<^sub>1 \<C>\<^sub>1 \<V>\<^sub>1 where
+    te_\<phi>1: "tseitin fresh \<V> \<phi>\<^sub>1 = (v\<^sub>1, ts\<^sub>1, \<C>\<^sub>1, \<V>\<^sub>1)"
+    using prod_cases4 by blast
+
+  obtain v\<^sub>2 ts\<^sub>2 \<C>\<^sub>2 \<V>\<^sub>2 where
+    te_\<phi>2: "tseitin fresh (\<V> \<union> \<V>\<^sub>1) \<phi>\<^sub>2 = (v\<^sub>2, ts\<^sub>2, \<C>\<^sub>2, \<V>\<^sub>2)"
+    using prod_cases4 by blast
+
+  define \<C>\<^sub>0 :: "('p \<times> ('v, 'f) fof_term list) literal list list" where
+    "\<C>\<^sub>0 = [
+      [Pos (v, []), Neg (v\<^sub>1, ts\<^sub>1)],
+      [Pos (v, []), Neg (v\<^sub>2, ts\<^sub>2)],
+      [Neg (v, []), Pos (v\<^sub>2, ts\<^sub>2), Pos (v\<^sub>1, ts\<^sub>1)]]"
+
+  have
+    "v = fresh (\<V> \<union> \<V>\<^sub>1 \<union> \<V>\<^sub>2)" and
+    "\<C> = \<C>\<^sub>0 @ \<C>\<^sub>1 @ \<C>\<^sub>2" and
+    "\<V>' = insert v (\<V>\<^sub>1 \<union> \<V>\<^sub>2)"
+    using Or.prems[simplified, unfolded te_\<phi>1, simplified, unfolded te_\<phi>2, simplified]
+    by (auto simp add: \<C>\<^sub>0_def Let_def)
+
+  have gen_var: 
+      "v \<in> predicates_of_formula (Or \<phi>\<^sub>1 \<phi>\<^sub>2) \<union> \<V>'"
+    by (simp add: \<open>\<V>' = insert v (\<V>\<^sub>1 \<union> \<V>\<^sub>2)\<close>)
+
+  have gen_vars_\<phi>1: 
+      "insert v\<^sub>1 (\<Union>C \<in> set \<C>\<^sub>1. fst ` atom ` set C) = predicates_of_formula \<phi>\<^sub>1 \<union> \<V>\<^sub>1"
+    using Or.IH(1)[OF te_\<phi>1]
+    by simp
+
+  have gen_vars_\<phi>2: 
+      "insert v\<^sub>2 (\<Union>C \<in> set \<C>\<^sub>2. fst ` atom ` set C) = predicates_of_formula \<phi>\<^sub>2 \<union> \<V>\<^sub>2"
+    using Or.IH(2)[OF te_\<phi>2]
+    by simp
+
+  have gen_vars: 
+      "insert v (\<Union>C \<in> set \<C>. fst ` atom ` set C) = predicates_of_formula (Or \<phi>\<^sub>1 \<phi>\<^sub>2) \<union> \<V>'"
+    unfolding \<open>\<C> = \<C>\<^sub>0 @ \<C>\<^sub>1 @ \<C>\<^sub>2\<close> \<C>\<^sub>0_def \<open>\<V>' = insert v (\<V>\<^sub>1 \<union> \<V>\<^sub>2)\<close>
+    using gen_vars_\<phi>1 gen_vars_\<phi>2
+    by fastforce
+
+  show ?case
+    using gen_var gen_vars
+    by simp
+qed
+
+fun formula_of_literal :: "('p \<times> ('v, 'f) fof_term list) literal \<Rightarrow> ('v, 'f, 'p) formula" where
+  "formula_of_literal (Pos (p, ts)) = Pred p ts" |
+  "formula_of_literal (Neg (p, ts)) = Not (Pred p ts)"
+
+definition formula_of_clause ::
+  "('p \<times> ('v, 'f) fof_term list) literal list \<Rightarrow> ('v, 'f, 'p) formula" where
+  "formula_of_clause Ls = fold (\<lambda>L. Or (formula_of_literal L)) Ls F"
+
+definition formula_of_clause_list ::
+  "('p \<times> ('v, 'f) fof_term list) literal list list \<Rightarrow> ('v, 'f, 'p) formula" where
+  "formula_of_clause_list Cs = fold (\<lambda>C. And (formula_of_clause C)) Cs T"
+
+lemma formula_of_clause_eq_fold_Or:
+  "formula_of_clause C = fold Or (map formula_of_literal C) F"
+  by (metis (no_types, lifting) ext comp_apply
+      fold_map formula_of_clause_def)
+
+lemma formula_of_clause_list_eq_fold_And:
+  "formula_of_clause_list Cs = fold And (map formula_of_clause Cs) T"
+  by (metis (no_types, lifting) ext comp_apply
+      fold_map formula_of_clause_list_def)
+
+lemma eval_formula_fold_And_iff:
+  "eval_formula (fold And xs \<phi>) vI fI pI \<longleftrightarrow>
+    eval_formula (fold And xs T) vI fI pI \<and> eval_formula \<phi> vI fI pI"
+proof (induction xs arbitrary: \<phi>)
+  case Nil
+  show ?case
+    by simp
+next
+  case (Cons a xs)
+  show ?case
+    by (metis eval_formula.simps(2)
+        fold_simps(2) local.Cons)
+qed
+
+lemma eval_formula_fold_And_append_iff:
+  "eval_formula (fold And (xs @ ys) \<phi>) vI fI pI \<longleftrightarrow>
+    eval_formula (fold And xs T) vI fI pI \<and>
+    eval_formula (fold And ys T) vI fI pI \<and>
+    eval_formula \<phi> vI fI pI"
+proof (induction xs)
+  case Nil
+  show ?case
+    by (metis append_self_conv2
+        eval_formula_fold_And_iff
+        fold_simps(1))
+next
+  case (Cons a xs)
+  show ?case
+    by (metis comp_apply
+        eval_formula_fold_And_iff
+        fold_append)
+qed
+
+lemma eval_formula_formula_of_clause_list_append_iff:
+  "eval_formula (formula_of_clause_list (xs @ ys)) vI fI pI \<longleftrightarrow>
+    eval_formula (formula_of_clause_list xs) vI fI pI \<and>
+    eval_formula (formula_of_clause_list ys) vI fI pI"
+proof (induction xs)
+  case Nil
+  show ?case
+    unfolding formula_of_clause_list_def formula_of_clause_def
+    by simp
+next
+  case (Cons a xs)
+
+  let ?xs = "map formula_of_clause xs"
+  let ?ys = "map formula_of_clause ys"
+  let ?a = "formula_of_clause a"
+
+  have "eval_formula (formula_of_clause_list ((a # xs) @ ys)) vI fI pI
+    \<longleftrightarrow> eval_formula (fold And (?xs @ ?ys) (And ?a T)) vI fI pI"
+    unfolding formula_of_clause_list_eq_fold_And
+    by simp
+  also have 
+      "... \<longleftrightarrow> eval_formula (fold And ?xs T) vI fI pI \<and> eval_formula (fold And ?ys T) vI fI pI \<and>
+               eval_formula (And ?a T) vI fI pI"
+    unfolding eval_formula_fold_And_append_iff
+    by simp
+  also have 
+      "... \<longleftrightarrow> (eval_formula (formula_of_clause_list (a # xs)) vI fI pI \<and>
+                    eval_formula (formula_of_clause_list ys) vI fI pI)"
+    by (metis calculation
+        eval_formula_fold_And_append_iff
+        eval_formula_fold_And_iff
+        formula_of_clause_list_eq_fold_And
+        map_append)
+  finally show ?case .
+qed
+
+lemma eval_formula_cong_wrt_predicate_evaluation:
+  assumes "\<And>x. x \<in> predicates_of_formula \<phi> \<Longrightarrow> pI x = pI' x"
+  shows "eval_formula \<phi> vI fI pI = eval_formula \<phi> vI fI pI'"
+  using assms
+proof (induction \<phi> arbitrary: vI)
+  case (Pred p args)
+  show ?case
+    by (simp add: Pred)
+next
+  case (And \<phi>1 \<phi>2)
+  show ?case 
+    by (simp add: And)
+next
+  case (Or \<phi>1 \<phi>2)
+  show ?case 
+    by (simp add: Or)
+next
+  case (Not \<phi>)
+  show ?case 
+    by (simp add: Not)
+next
+  case (Equal t1 t2)
+  show ?case 
+    by (simp add: Equal)
+next
+  case (Forall v \<phi>)
+  have preds_of_\<phi>: "\<And>p. p \<in> predicates_of_formula \<phi> \<Longrightarrow> pI p = pI' p"
+    by (simp add: Forall.prems)
+  show ?case
+    using Forall.IH preds_of_\<phi> 
+    by auto
+next
+  case (Exists v \<phi>)
+  have preds_of_\<phi>: "\<And>p. p \<in> predicates_of_formula \<phi> \<Longrightarrow> pI p = pI' p"
+    by (simp add: Exists.prems)
+  show ?case
+    using Exists.IH preds_of_\<phi> 
+    by auto
+next
+  case T
+  show ?case
+    by simp
+next
+  case F
+  show ?case
+    by simp
+qed
+
+lemma predicates_of_formula_of_literal:
+  "predicates_of_formula (formula_of_literal l) = fst ` atom ` {l}"
+proof (cases l)
+  case (Pos pred)
+  obtain p ts where "pred = (p, ts)"
+    by fastforce
+  show ?thesis
+    by (simp add: Pos \<open>pred = (p, ts)\<close>)
+next
+  case (Neg pred)
+  obtain p ts where "pred = (p, ts)"
+    by fastforce
+  show ?thesis
+    using Neg \<open>pred = (p, ts)\<close> by auto
+qed
+
+lemma predicates_of_formula_fold_Or_map_formula_of_literal:
+  "predicates_of_formula (fold Or (map formula_of_literal C) \<phi>) =
+  fst ` atom ` set C \<union> predicates_of_formula \<phi>"
+proof (induction C arbitrary: \<phi>)
+  case Nil
+  show ?case
+    by simp
+next
+  case (Cons a C)
+
+  have clause_simp: "fold Or (map formula_of_literal (a # C)) \<phi>
+    = fold Or (map formula_of_literal C) (Or (formula_of_literal a) \<phi>)"
+    by simp
+
+  have "predicates_of_formula (fold Or (map formula_of_literal (a # C)) \<phi>)
+    = fst ` atom ` set C \<union> predicates_of_formula (Or (formula_of_literal a) \<phi>)"
+    unfolding clause_simp
+    using Cons.IH
+    by simp
+  also have "... = fst ` atom ` set C \<union> 
+    predicates_of_formula (formula_of_literal a) \<union> predicates_of_formula \<phi>"
+    by auto
+  also have "... = fst ` atom ` set C \<union> fst ` atom ` {a} \<union> predicates_of_formula \<phi>"
+    by (simp add: predicates_of_formula_of_literal)
+  also have "... = fst ` atom ` set (a # C) \<union> predicates_of_formula \<phi>"
+    by simp
+  finally show ?case .
+qed
+
+lemma predicates_of_formula_of_clause:
+  "predicates_of_formula (formula_of_clause C) = fst ` atom ` set C"
+proof (induction C)
+  case Nil
+  show ?case
+    unfolding formula_of_clause_def
+    by simp
+next
+  case (Cons a C)
+  have "predicates_of_formula (formula_of_clause (a # C))
+    = predicates_of_formula (fold Or (map formula_of_literal C) (Or (formula_of_literal a) F))"
+    unfolding formula_of_clause_eq_fold_Or
+    by simp
+  also have "... = predicates_of_formula (formula_of_clause C) \<union> 
+                   predicates_of_formula (formula_of_literal a) "
+    unfolding predicates_of_formula_fold_Or_map_formula_of_literal
+    by (simp add: local.Cons)
+  also have "... = fst ` atom ` set C \<union> fst ` atom ` {a}"
+    by (simp add: local.Cons predicates_of_formula_of_literal)
+  also have "... = fst ` atom ` set (a # C)"
+    by simp
+  finally show ?case .
+qed
+
+lemma predicates_of_formula_fold_And_map_formula_of_clause:
+  "predicates_of_formula (fold And (map formula_of_clause Cs) \<phi>) =
+  (\<Union> C \<in> set Cs. predicates_of_formula (formula_of_clause C)) \<union> predicates_of_formula \<phi>"
+proof (induction Cs arbitrary: \<phi>)
+  case Nil
+  show ?case
+    by simp
+next
+  case (Cons a Cs)
+
+  have clause_list_simp: "fold And (map formula_of_clause (a # Cs)) \<phi>
+    = (fold And (map formula_of_clause Cs) (And (formula_of_clause a) \<phi>))"
+    by simp
+
+  have "predicates_of_formula (fold And (map formula_of_clause (a # Cs)) \<phi>)
+    = (\<Union> C \<in> set Cs. predicates_of_formula (formula_of_clause C)) \<union>
+      predicates_of_formula (And (formula_of_clause a) \<phi>)"
+    unfolding clause_list_simp
+    using Cons.IH
+    by simp
+  also have "... = (\<Union> C \<in> set Cs. predicates_of_formula (formula_of_clause C)) \<union>
+      predicates_of_formula (formula_of_clause a) \<union>
+      predicates_of_formula  \<phi>"
+    by auto
+  also have "... = (\<Union>C\<in>set (a # Cs). 
+      predicates_of_formula (formula_of_clause C)) \<union> predicates_of_formula \<phi>"
+    by auto
+  finally show ?case .
+qed
+
+lemma predicates_of_formula_of_clause_list:
+  "predicates_of_formula (formula_of_clause_list Cs) =
+    (\<Union> C \<in> set Cs. predicates_of_formula (formula_of_clause C))"
+proof (induction Cs)
+  case Nil
+  show ?case
+    unfolding formula_of_clause_list_def formula_of_clause_def
+    by simp
+next
+  case (Cons a Cs)
+  have "predicates_of_formula (formula_of_clause_list (a # Cs))
+    = predicates_of_formula (fold And (map formula_of_clause Cs) (And (formula_of_clause a) T))"
+    unfolding formula_of_clause_list_eq_fold_And
+    by simp
+  also have "... = (\<Union>C\<in>set (a # Cs). predicates_of_formula (formula_of_clause C))"
+    unfolding predicates_of_formula_fold_And_map_formula_of_clause
+    by auto
+  finally show ?case .
+qed
+
+theorem tseitin_spec:
+  fixes fresh :: "'p set \<Rightarrow> 'p"
+  assumes fresh_spec: "\<And>\<V>. finite \<V> \<Longrightarrow> fresh \<V> \<notin> \<V>"
+  fixes \<phi> :: "('v, 'f, 'p) formula"
+  assumes "is_nnf \<phi>"
+  assumes "finite \<V>" and "predicates_of_formula \<phi> \<subseteq> \<V>"
+  assumes tseitin: "tseitin fresh \<V> \<phi> = (v, ts, \<C>, \<V>')"
+  fixes pI :: "'p \<Rightarrow> 'd list \<Rightarrow> bool"
+  shows "\<exists>pI'.
+    (\<forall>x \<in> predicates_of_formula \<phi>. pI' x = pI x) \<and>
+    eval_formula (formula_of_clause_list \<C>) vI fI pI' \<and>
+    (eval_formula (Pred v ts) vI fI pI' \<longleftrightarrow> eval_formula \<phi> vI fI pI)"
+  using \<open>is_nnf \<phi>\<close> \<open>finite \<V>\<close> \<open>predicates_of_formula \<phi> \<subseteq> \<V>\<close> tseitin
+proof (induction \<phi> arbitrary: \<V> v ts \<C> \<V>' rule: is_nnf.induct)
+  case (PosPred p ts\<^sub>p)
+
+  have  "v = p" and
+        "ts = ts\<^sub>p" and
+        "\<C> = []" and
+        "\<V>' = {}"
+    unfolding atomize_conj
+    using PosPred.prems[simplified]
+    by (auto simp add: Let_def)
+
+  define pI' :: "'p \<Rightarrow> 'd list \<Rightarrow> bool" where
+    "pI' = pI"
+
+  show ?case
+  proof (intro exI conjI ballI)
+    show "\<And>x. x \<in> predicates_of_formula (Pred p ts\<^sub>p) \<Longrightarrow> pI' x = pI x"
+      unfolding pI'_def
+      by simp
+  next
+    show "eval_formula (formula_of_clause_list \<C>) vI fI pI'"
+      unfolding \<open>\<C> = []\<close> formula_of_clause_list_def
+      by simp
+  next
+    show "eval_formula (Pred v ts) vI fI pI' \<longleftrightarrow> eval_formula (Pred p ts\<^sub>p) vI fI pI"
+      unfolding pI'_def \<open>v = p\<close> \<open>ts = ts\<^sub>p\<close>
+      by simp
+  qed
+next
+  case (NegPred p ts\<^sub>p)
+
+  define \<C>\<^sub>0 :: "('p \<times> ('v, 'f) fof_term list) literal list list" where
+    "\<C>\<^sub>0 = [
+      [Neg (v, []), Neg (p, ts\<^sub>p)],
+      [Pos (v, []), Pos (p, ts\<^sub>p)]]"
+
+  have "v = fresh \<V>" and
+       "ts = []" and
+       "\<C> = \<C>\<^sub>0" and
+       "\<V>' = insert v {}"
+    unfolding atomize_conj
+    using NegPred.prems[simplified]
+    by (metis Pair_inject \<C>\<^sub>0_def)
+
+  define pI' :: "'p \<Rightarrow> 'd list \<Rightarrow> bool" where
+    "pI' = (\<lambda>x ds. if x = v then \<not> pI p (map (\<lambda>t. eval_term t vI fI) ts\<^sub>p) else pI x ds)"
+
+  show ?case
+  proof (intro exI conjI ballI)
+    show "\<And>x. x \<in> predicates_of_formula (formula.Not (Pred p ts\<^sub>p)) \<Longrightarrow> pI' x = pI x"
+      unfolding pI'_def
+      using NegPred.prems(1,2) \<open>v = fresh \<V>\<close> fresh_spec 
+      by auto
+  next
+    show "eval_formula (formula_of_clause_list \<C>) vI fI pI'"
+      unfolding \<open>\<C> = \<C>\<^sub>0\<close>
+    proof -
+      have simp1: "formula_of_clause_list \<C>\<^sub>0
+        = And (Or (Pred p ts\<^sub>p) (Or (Pred v ts) F))
+              (And (Or (Not (Pred p ts\<^sub>p)) (Or (Not (Pred v ts)) F)) T)"
+        unfolding \<C>\<^sub>0_def formula_of_clause_list_def formula_of_clause_def \<open>ts = []\<close>
+        by simp
+      have simp2: "eval_formula (formula_of_clause_list \<C>\<^sub>0) vI fI pI'
+        = eval_formula 
+          (And (Or (Pred p ts\<^sub>p) (Pred v ts)) 
+               (Or (Not (Pred p ts\<^sub>p)) (Not (Pred v ts)))) vI fI pI'"
+        using \<open>ts = []\<close>
+        by (simp add: simp1)
+
+      have posv: "eval_formula (Pred v ts) vI fI pI'
+        = (\<not> pI p (map (\<lambda>t. eval_term t vI fI) ts\<^sub>p))"
+        unfolding pI'_def
+        by simp
+      have negv: "eval_formula (Not (Pred v ts)) vI fI pI'
+        = pI p (map (\<lambda>t. eval_term t vI fI) ts\<^sub>p)"
+        unfolding pI'_def
+        by simp
+      have pospred: "eval_formula (Pred p ts\<^sub>p) vI fI pI'
+        = pI p (map (\<lambda>t. eval_term t vI fI) ts\<^sub>p)"
+        unfolding eval_formula.simps pI'_def
+        using NegPred.prems(1,2) \<open>v = fresh \<V>\<close> fresh_spec 
+        by force
+      have negpred: "eval_formula (Not (Pred p ts\<^sub>p)) vI fI pI'
+        = (\<not> pI p (map (\<lambda>t. eval_term t vI fI) ts\<^sub>p))"
+        unfolding eval_formula.simps pI'_def
+        using NegPred.prems(1,2) \<open>v = fresh \<V>\<close> fresh_spec 
+        by force
+
+      show "eval_formula (formula_of_clause_list \<C>\<^sub>0) vI fI pI'"
+        using simp2 pospred posv negpred negv
+        by auto
+    qed
+  next
+    show "eval_formula (Pred v ts) vI fI pI' \<longleftrightarrow> eval_formula (formula.Not (Pred p ts\<^sub>p)) vI fI pI"
+      unfolding eval_formula.simps pI'_def
+      by simp
+  qed
+next
+  case Connective: (And \<phi>\<^sub>1 \<phi>\<^sub>2)
+  obtain v\<^sub>1 ts\<^sub>1 \<C>\<^sub>1 \<V>\<^sub>1 where
+    te_\<phi>1: "tseitin fresh \<V> \<phi>\<^sub>1 = (v\<^sub>1, ts\<^sub>1, \<C>\<^sub>1, \<V>\<^sub>1)"
+    using prod_cases4 by blast
+
+  obtain v\<^sub>2 ts\<^sub>2 \<C>\<^sub>2 \<V>\<^sub>2 where
+    te_\<phi>2: "tseitin fresh (\<V> \<union> \<V>\<^sub>1) \<phi>\<^sub>2 = (v\<^sub>2, ts\<^sub>2, \<C>\<^sub>2, \<V>\<^sub>2)"
+    using prod_cases4 by blast
+
+  define \<C>\<^sub>0 :: "('p \<times> ('v, 'f) fof_term list) literal list list" where
+    "\<C>\<^sub>0 = [
+      [Neg (v, []), Pos (v\<^sub>1, ts\<^sub>1)], 
+      [Neg (v, []), Pos (v\<^sub>2, ts\<^sub>2)], 
+      [Pos (v, []), Neg (v\<^sub>1, ts\<^sub>1), Neg (v\<^sub>2, ts\<^sub>2)]]"
+
+  have
+    "v = fresh (\<V> \<union> \<V>\<^sub>1 \<union> \<V>\<^sub>2)" and
+    "\<C> = \<C>\<^sub>0 @ \<C>\<^sub>1 @ \<C>\<^sub>2" and
+    "\<V>' = insert v (\<V>\<^sub>1 \<union> \<V>\<^sub>2)"
+    using Connective.prems[simplified, unfolded te_\<phi>1, simplified, unfolded te_\<phi>2, simplified]
+    by (auto simp add: \<C>\<^sub>0_def Let_def)
+
+  obtain pI1 where
+    pI1_extends_pI: "\<forall>x\<in>predicates_of_formula \<phi>\<^sub>1. pI1 x = pI x" and
+    pI1_model: "eval_formula (formula_of_clause_list \<C>\<^sub>1) vI fI pI1" and
+    v\<^sub>1_equisat_\<phi>\<^sub>1: "eval_formula (Pred v\<^sub>1 ts\<^sub>1) vI fI pI1 \<longleftrightarrow> eval_formula \<phi>\<^sub>1 vI fI pI"
+    using Connective.IH(1)[OF _ _ te_\<phi>1] Connective.prems(1,2) 
+    by auto
+
+  obtain pI2 where
+    pI2_extends_pI: "\<forall>x\<in>predicates_of_formula \<phi>\<^sub>2. pI2 x = pI x" and
+    pI2_model: "eval_formula (formula_of_clause_list \<C>\<^sub>2) vI fI pI2" and
+    v\<^sub>2_equisat_\<phi>\<^sub>2: "eval_formula (Pred v\<^sub>2 ts\<^sub>2) vI fI pI2 \<longleftrightarrow> eval_formula \<phi>\<^sub>2 vI fI pI"
+    using Connective.IH(2)[OF _ _ te_\<phi>2] te_\<phi>1 Connective.prems(1,2)
+    by (metis (no_types, lifting) Connective.hyps(1)
+        finite_Un formula.simps(207) le_sup_iff
+        sup.coboundedI2 sup_commute
+        tseitin_finite_var_set)
+
+  define pI' :: "'p \<Rightarrow> 'd list \<Rightarrow> bool" where
+    "pI' = (\<lambda>x ds. 
+      if x = v then pI1 v\<^sub>1 (map (\<lambda>t. eval_term t vI fI) ts\<^sub>1) \<and> pI2 v\<^sub>2 (map (\<lambda>t. eval_term t vI fI) ts\<^sub>2) 
+      else (if x \<in> \<V>\<^sub>1 then pI1 x ds 
+      else (if x \<in> \<V>\<^sub>2 then pI2 x ds 
+      else pI x ds)))"
+
+  have "v\<^sub>1 \<in> predicates_of_formula \<phi>\<^sub>1 \<union> \<V>\<^sub>1"
+    using tseitin_generated_var[OF _ te_\<phi>1]
+    by (simp add: Connective.hyps(1))
+
+  have "v\<^sub>2 \<in> predicates_of_formula \<phi>\<^sub>2 \<union> \<V>\<^sub>2"
+    using tseitin_generated_var[OF _ te_\<phi>2]
+    by (simp add: Connective.hyps(2))
+
+  have "\<V> \<inter> \<V>\<^sub>1 = {}"
+    using tseitin_fresh_vars[OF fresh_spec \<open>is_nnf \<phi>\<^sub>1\<close> \<open>finite \<V>\<close> te_\<phi>1]
+    by simp
+
+  have "finite (\<V> \<union> \<V>\<^sub>1)"
+  proof -
+    have "finite \<V>\<^sub>1"
+      using tseitin_finite_var_set[OF \<open>is_nnf \<phi>\<^sub>1\<close> te_\<phi>1]
+      by simp
+    show ?thesis
+      using \<open>finite \<V>\<close> \<open>finite \<V>\<^sub>1\<close>
+      by simp
+  qed
+
+  have "(\<V> \<union> \<V>\<^sub>1) \<inter> \<V>\<^sub>2 = {}"
+    using tseitin_fresh_vars[OF fresh_spec \<open>is_nnf \<phi>\<^sub>2\<close> \<open>finite (\<V> \<union> \<V>\<^sub>1)\<close> te_\<phi>2]
+    by simp
+
+  have "finite (\<V> \<union> \<V>\<^sub>1 \<union> \<V>\<^sub>2)"
+  proof -
+    have "finite \<V>\<^sub>2"
+      using tseitin_finite_var_set[OF \<open>is_nnf \<phi>\<^sub>2\<close> te_\<phi>2]
+      by simp
+    show ?thesis
+      using \<open>finite (\<V> \<union> \<V>\<^sub>1)\<close> \<open>finite \<V>\<^sub>2\<close>
+      by simp
+  qed
+
+  have "v \<in> \<V>'" and "v \<notin> (\<V> \<union> \<V>\<^sub>1 \<union> \<V>\<^sub>2)"
+    unfolding atomize_conj
+  proof (rule conjI)
+    show "v \<in> \<V>'"
+      by (simp add: \<open>\<V>' = insert v (\<V>\<^sub>1 \<union> \<V>\<^sub>2)\<close>)
+  next
+    show "v \<notin> (\<V> \<union> \<V>\<^sub>1 \<union> \<V>\<^sub>2)"
+      unfolding \<open>v = fresh (\<V> \<union> \<V>\<^sub>1 \<union> \<V>\<^sub>2)\<close>
+      using fresh_spec[OF \<open>finite (\<V> \<union> \<V>\<^sub>1 \<union> \<V>\<^sub>2)\<close>]
+      by simp
+  qed
+
+  show ?case
+  proof (intro exI conjI ballI)
+    fix x
+    assume preds: "x \<in> predicates_of_formula (And \<phi>\<^sub>1 \<phi>\<^sub>2)"
+    have "x \<in> \<V>"
+      using preds Connective.prems(2)
+      by blast
+    have x_ne_v: "x \<noteq> v"
+      using \<open>v = fresh (\<V> \<union> \<V>\<^sub>1 \<union> \<V>\<^sub>2)\<close> \<open>x \<in> \<V>\<close> fresh_spec
+      by (meson Connective.hyps(1,2)
+          Connective.prems(1) UnCI finite_UnI te_\<phi>1
+          te_\<phi>2 tseitin_finite_var_set)
+    have x_ni_\<V>': "x \<in> \<V> \<Longrightarrow> x \<notin> \<V>'"
+      by (metis And Connective.hyps(1,2)
+          Connective.prems(1,3) IntI empty_iff 
+          fresh_spec tseitin_fresh_vars)
+    have x_ni_\<V>1: "x \<notin> \<V>\<^sub>1" and x_ni_\<V>2: "x \<notin> \<V>\<^sub>2"
+      using \<open>\<V>' = insert v (\<V>\<^sub>1 \<union> \<V>\<^sub>2)\<close> \<open>x \<in> \<V>\<close> x_ni_\<V>'
+      by auto
+    show "pI' x = pI x"
+      unfolding pI'_def
+      using x_ne_v x_ni_\<V>1 x_ni_\<V>2
+      by auto 
+  next
+    show "eval_formula (formula_of_clause_list \<C>) vI fI pI'"
+      unfolding \<open>\<C> = \<C>\<^sub>0 @ \<C>\<^sub>1 @ \<C>\<^sub>2\<close> eval_formula_formula_of_clause_list_append_iff
+    proof(intro conjI)
+
+      have simp1: "formula_of_clause_list \<C>\<^sub>0 = 
+        And (Or (Not (Pred v\<^sub>2 ts\<^sub>2)) (Or (Not (Pred v\<^sub>1 ts\<^sub>1)) (Or (Pred v []) F)))
+            (And (Or (Pred v\<^sub>2 ts\<^sub>2) (Or (Not (Pred v [])) F))
+                 (And (Or (Pred v\<^sub>1 ts\<^sub>1) (Or (Not (Pred v [])) F)) T))" 
+        unfolding \<C>\<^sub>0_def formula_of_clause_list_def formula_of_clause_def
+        by simp
+
+      have simp2: "eval_formula (formula_of_clause_list \<C>\<^sub>0) vI fI pI'
+        = eval_formula
+          (And (Or (Not (Pred v\<^sub>2 ts\<^sub>2)) (Or (Not (Pred v\<^sub>1 ts\<^sub>1)) (Pred v [])))
+               (And (Or (Pred v\<^sub>2 ts\<^sub>2) (Not (Pred v [])))
+                    (Or (Pred v\<^sub>1 ts\<^sub>1) (Not (Pred v []))))) vI fI pI'"
+        unfolding simp1
+        by simp
+
+      have posv: "eval_formula (Pred v []) vI fI pI'
+        = (pI1 v\<^sub>1 (map (\<lambda>t. eval_term t vI fI) ts\<^sub>1) \<and> pI2 v\<^sub>2 (map (\<lambda>t. eval_term t vI fI) ts\<^sub>2))"
+        unfolding pI'_def
+        by simp
+      have negv: "eval_formula (Not (Pred v [])) vI fI pI'
+        = (\<not> (pI1 v\<^sub>1 (map (\<lambda>t. eval_term t vI fI) ts\<^sub>1) \<and> pI2 v\<^sub>2 (map (\<lambda>t. eval_term t vI fI) ts\<^sub>2)))"
+        using posv
+        by simp
+
+      have posv1: "v\<^sub>1 \<in> \<V>\<^sub>1 \<Longrightarrow> 
+        (eval_formula (Pred v\<^sub>1 ts\<^sub>1) vI fI pI' = pI1 v\<^sub>1 (map (\<lambda>t. eval_term t vI fI) ts\<^sub>1))"
+        unfolding eval_formula.simps pI'_def
+        using \<open>v \<notin> (\<V> \<union> \<V>\<^sub>1 \<union> \<V>\<^sub>2)\<close> 
+        by auto
+      have negv1: "v\<^sub>1 \<in> \<V>\<^sub>1 \<Longrightarrow> 
+        (eval_formula (Not (Pred v\<^sub>1 ts\<^sub>1)) vI fI pI' = (\<not> pI1 v\<^sub>1 (map (\<lambda>t. eval_term t vI fI) ts\<^sub>1)))" 
+        using posv1 
+        by auto
+
+      have posv2: "v\<^sub>2 \<in> \<V>\<^sub>2 \<Longrightarrow> 
+        (eval_formula (Pred v\<^sub>2 ts\<^sub>2) vI fI pI' = pI2 v\<^sub>2 (map (\<lambda>t. eval_term t vI fI) ts\<^sub>2))"
+      proof -
+        assume "v\<^sub>2 \<in> \<V>\<^sub>2"
+        have "v\<^sub>2 \<notin> \<V>" and "v\<^sub>2 \<notin> \<V>\<^sub>1"
+          unfolding atomize_conj
+          using \<open>v\<^sub>2 \<in> \<V>\<^sub>2\<close> \<open>(\<V> \<union> \<V>\<^sub>1) \<inter> \<V>\<^sub>2 = {}\<close> 
+          by auto
+        have "v\<^sub>2 \<noteq> v"
+          using \<open>v\<^sub>2 \<in> \<V>\<^sub>2\<close> \<open>v \<notin> (\<V> \<union> \<V>\<^sub>1 \<union> \<V>\<^sub>2)\<close>
+          by auto
+        show ?thesis
+          unfolding eval_formula.simps pI'_def
+          by (simp add: \<open>v\<^sub>2 \<in> \<V>\<^sub>2\<close> \<open>v\<^sub>2 \<noteq> v\<close> \<open>v\<^sub>2 \<notin> \<V>\<^sub>1\<close>)
+      qed
+      have negv2: "v\<^sub>2 \<in> \<V>\<^sub>2 \<Longrightarrow> 
+        (eval_formula (Not (Pred v\<^sub>2 ts\<^sub>2)) vI fI pI' = (\<not> pI2 v\<^sub>2 (map (\<lambda>t. eval_term t vI fI) ts\<^sub>2)))"
+        using posv2 
+        by auto
+
+      have posv1_pred: "v\<^sub>1 \<in> predicates_of_formula \<phi>\<^sub>1 \<Longrightarrow> 
+        (eval_formula (Pred v\<^sub>1 ts\<^sub>1) vI fI pI' = pI v\<^sub>1 (map (\<lambda>t. eval_term t vI fI) ts\<^sub>1))"
+      proof -
+        assume assumption: "v\<^sub>1 \<in> predicates_of_formula \<phi>\<^sub>1"
+        have pred_\<phi>1_in_\<V>: "predicates_of_formula \<phi>\<^sub>1 \<subseteq> \<V>"
+          using Connective.prems(2) 
+          by auto
+        have "v\<^sub>1 \<in> \<V>"
+          using assumption pred_\<phi>1_in_\<V>
+          by auto
+        have "v\<^sub>1 \<notin> \<V>\<^sub>1"
+          using \<open>v\<^sub>1 \<in> \<V>\<close> \<open>\<V> \<inter> \<V>\<^sub>1 = {}\<close>
+          by auto
+        have "v\<^sub>1 \<notin> \<V>\<^sub>2"
+          using \<open>v\<^sub>1 \<in> \<V>\<close> \<open>(\<V> \<union> \<V>\<^sub>1) \<inter> \<V>\<^sub>2 = {}\<close>
+          by auto
+        have "v\<^sub>1 \<noteq> v"
+          using \<open>v\<^sub>1 \<in> \<V>\<close> \<open>v \<notin> (\<V> \<union> \<V>\<^sub>1 \<union> \<V>\<^sub>2)\<close> 
+          by auto
+        show ?thesis
+          unfolding eval_formula.simps pI'_def
+          by (simp add: \<open>v\<^sub>1 \<noteq> v\<close> \<open>v\<^sub>1 \<notin> \<V>\<^sub>1\<close> \<open>v\<^sub>1 \<notin> \<V>\<^sub>2\<close>)
+      qed
+      have negv1_pred: "v\<^sub>1 \<in> predicates_of_formula \<phi>\<^sub>1 \<Longrightarrow> 
+        (eval_formula (Not (Pred v\<^sub>1 ts\<^sub>1)) vI fI pI' = (\<not> pI v\<^sub>1 (map (\<lambda>t. eval_term t vI fI) ts\<^sub>1)))"
+        using posv1_pred 
+        by auto
+
+      have posv2_pred: "v\<^sub>2 \<in> predicates_of_formula \<phi>\<^sub>2 \<Longrightarrow> 
+        (eval_formula (Pred v\<^sub>2 ts\<^sub>2) vI fI pI' = pI v\<^sub>2 (map (\<lambda>t. eval_term t vI fI) ts\<^sub>2))"
+      proof -
+        assume assumption: "v\<^sub>2 \<in> predicates_of_formula \<phi>\<^sub>2"
+        have pred_\<phi>2_in_\<V>: "predicates_of_formula \<phi>\<^sub>2 \<subseteq> \<V>"
+          using Connective.prems(2)
+          by auto
+        have "v\<^sub>2 \<in> \<V>"
+          using assumption pred_\<phi>2_in_\<V>
+          by auto
+        have "v\<^sub>2 \<notin> \<V>\<^sub>1"
+          using \<open>v\<^sub>2 \<in> \<V>\<close> \<open>\<V> \<inter> \<V>\<^sub>1 = {}\<close>
+          by auto
+        have "v\<^sub>2 \<notin> \<V>\<^sub>2"
+          using \<open>v\<^sub>2 \<in> \<V>\<close> \<open>(\<V> \<union> \<V>\<^sub>1) \<inter> \<V>\<^sub>2 = {}\<close>
+          by auto
+        have "v\<^sub>2 \<noteq> v"
+          using \<open>v\<^sub>2 \<in> \<V>\<close> \<open>v \<notin> (\<V> \<union> \<V>\<^sub>1 \<union> \<V>\<^sub>2)\<close>
+          by auto
+        show ?thesis
+          unfolding eval_formula.simps pI'_def
+          by (simp add: \<open>v\<^sub>2 \<noteq> v\<close> \<open>v\<^sub>2 \<notin> \<V>\<^sub>1\<close> \<open>v\<^sub>2 \<notin> \<V>\<^sub>2\<close>)
+      qed
+      have negv2_pred: "v\<^sub>2 \<in> predicates_of_formula \<phi>\<^sub>2 \<Longrightarrow> 
+        (eval_formula (Not (Pred v\<^sub>2 ts\<^sub>2)) vI fI pI' = (\<not> pI v\<^sub>2 (map (\<lambda>t. eval_term t vI fI) ts\<^sub>2)))"
+        using posv2_pred 
+        by auto
+
+      consider
+        (A) "v\<^sub>1 \<in> predicates_of_formula \<phi>\<^sub>1 \<and> (v\<^sub>2 \<in> predicates_of_formula \<phi>\<^sub>2)" |
+        (B) "v\<^sub>1 \<in> predicates_of_formula \<phi>\<^sub>1 \<and> (v\<^sub>2 \<in> \<V>\<^sub>2)" |
+        (C) "v\<^sub>1 \<in> \<V>\<^sub>1 \<and> (v\<^sub>2 \<in> predicates_of_formula \<phi>\<^sub>2)" |
+        (D) "v\<^sub>1 \<in> \<V>\<^sub>1 \<and> (v\<^sub>2 \<in> \<V>\<^sub>2)"
+        using
+          \<open>v\<^sub>1 \<in> predicates_of_formula \<phi>\<^sub>1 \<union> \<V>\<^sub>1\<close>
+          \<open>v\<^sub>2 \<in> predicates_of_formula \<phi>\<^sub>2 \<union> \<V>\<^sub>2\<close>
+        by blast
+
+      then show "eval_formula (formula_of_clause_list \<C>\<^sub>0) vI fI pI'"
+      proof cases
+        case A
+        then show ?thesis
+          unfolding simp2
+          using posv posv1_pred posv2_pred pI1_extends_pI pI2_extends_pI
+          by simp
+      next
+        case B
+        then show ?thesis
+          unfolding simp2
+          using posv negv2 posv1_pred pI1_extends_pI
+          by simp
+      next
+        case C
+        then show ?thesis 
+          unfolding simp2
+          using posv negv1 posv2_pred pI2_extends_pI
+          by simp
+      next
+        case D
+        then show ?thesis
+          unfolding simp2
+          using posv posv1 posv2
+          by simp
+      qed
+    next
+      show "eval_formula (formula_of_clause_list \<C>\<^sub>1) vI fI pI'"
+      proof (rule eval_formula_cong_wrt_predicate_evaluation[THEN iffD1, of _ pI1])
+        fix x
+        assume assumption: "x \<in> predicates_of_formula (formula_of_clause_list \<C>\<^sub>1)"
+
+        have ins_v: "insert v\<^sub>1 (predicates_of_formula (formula_of_clause_list \<C>\<^sub>1))
+          = predicates_of_formula \<phi>\<^sub>1 \<union> \<V>\<^sub>1"
+          unfolding predicates_of_formula_of_clause_list
+          unfolding predicates_of_formula_of_clause
+          using tseitin_generated_vars[OF \<open>is_nnf \<phi>\<^sub>1\<close> te_\<phi>1]
+          by simp
+
+        have x_in: "x \<in> predicates_of_formula \<phi>\<^sub>1 \<union> \<V>\<^sub>1"
+          using assumption ins_v
+          by auto
+
+        have x_in_preds: "x \<in> predicates_of_formula \<phi>\<^sub>1 \<Longrightarrow> pI1 x = pI' x" 
+        proof -
+          assume assm: "x \<in> predicates_of_formula \<phi>\<^sub>1"
+          have "x \<in> \<V>"
+          proof -
+            have "predicates_of_formula \<phi>\<^sub>1 \<subseteq> predicates_of_formula (And \<phi>\<^sub>1 \<phi>\<^sub>2)"
+              by simp
+            also have subset: "... \<subseteq> \<V>"
+              using \<open>predicates_of_formula (And \<phi>\<^sub>1 \<phi>\<^sub>2) \<subseteq> \<V>\<close>
+              by simp
+            show ?thesis
+              using subset assm
+              by auto
+          qed
+          have "x \<notin> \<V>\<^sub>2"
+            using \<open>x \<in> \<V>\<close> \<open>(\<V> \<union> \<V>\<^sub>1) \<inter> \<V>\<^sub>2 = {}\<close>
+            by auto
+          have "x \<noteq> v"
+            using \<open>x \<in> \<V>\<close> \<open>v \<notin> (\<V> \<union> \<V>\<^sub>1 \<union> \<V>\<^sub>2)\<close> 
+            by auto
+          show ?thesis
+            unfolding pI'_def
+            using \<open>x \<noteq> v\<close> \<open>x \<notin> \<V>\<^sub>2\<close> assm pI1_extends_pI 
+            by simp
+        qed
+
+        have x_in_\<V>1: "x \<in> \<V>\<^sub>1 \<Longrightarrow> pI1 x = pI' x"
+        proof -
+          assume "x \<in> \<V>\<^sub>1"
+          have "x \<noteq> v"
+            using \<open>x \<in> \<V>\<^sub>1\<close> \<open>v \<notin> (\<V> \<union> \<V>\<^sub>1 \<union> \<V>\<^sub>2)\<close>
+            by auto
+          show ?thesis
+            unfolding pI'_def
+            using \<open>x \<noteq> v\<close> \<open>x \<in> \<V>\<^sub>1\<close>
+            by simp
+        qed
+
+        show "pI1 x = pI' x"
+          using x_in x_in_preds x_in_\<V>1
+          by blast
+      next
+        show "eval_formula (formula_of_clause_list \<C>\<^sub>1) vI fI pI1"
+          by (simp add: pI1_model)
+      qed
+    next
+      show "eval_formula (formula_of_clause_list \<C>\<^sub>2) vI fI pI'"
+      proof (rule eval_formula_cong_wrt_predicate_evaluation[THEN iffD1, of _ pI2])
+        fix x
+        assume assumption: "x \<in> predicates_of_formula (formula_of_clause_list \<C>\<^sub>2)"
+
+        have ins_v: "insert v\<^sub>2 (predicates_of_formula (formula_of_clause_list \<C>\<^sub>2))
+          = predicates_of_formula \<phi>\<^sub>2 \<union> \<V>\<^sub>2"
+          unfolding predicates_of_formula_of_clause_list
+          unfolding predicates_of_formula_of_clause
+          using tseitin_generated_vars[OF \<open>is_nnf \<phi>\<^sub>2\<close> te_\<phi>2]
+          by simp
+
+        have x_in: "x \<in> predicates_of_formula \<phi>\<^sub>2 \<union> \<V>\<^sub>2"
+          using assumption ins_v
+          by auto
+
+        have x_in_preds: "x \<in> predicates_of_formula \<phi>\<^sub>2 \<Longrightarrow> pI2 x = pI' x" 
+        proof -
+          assume assm: "x \<in> predicates_of_formula \<phi>\<^sub>2"
+          have "x \<in> \<V>"
+          proof -
+            have "predicates_of_formula \<phi>\<^sub>2 \<subseteq> predicates_of_formula (And \<phi>\<^sub>1 \<phi>\<^sub>2)"
+              by simp
+            also have subset: "... \<subseteq> \<V>"
+              using \<open>predicates_of_formula (And \<phi>\<^sub>1 \<phi>\<^sub>2) \<subseteq> \<V>\<close>
+              by simp
+            show ?thesis
+              using subset assm
+              by auto
+          qed
+          have "x \<notin> \<V>\<^sub>1"
+            using \<open>x \<in> \<V>\<close> \<open>\<V> \<inter> \<V>\<^sub>1 = {}\<close>
+            by auto
+          have "x \<noteq> v"
+            using \<open>x \<in> \<V>\<close> \<open>v \<notin> (\<V> \<union> \<V>\<^sub>1 \<union> \<V>\<^sub>2)\<close> 
+            by auto
+          show ?thesis
+            unfolding pI'_def
+            using \<open>x \<noteq> v\<close> \<open>x \<notin> \<V>\<^sub>1\<close> assm pI2_extends_pI
+            by simp
+        qed
+
+        have x_in_\<V>2: "x \<in> \<V>\<^sub>2 \<Longrightarrow> pI2 x = pI' x"
+        proof -
+          assume "x \<in> \<V>\<^sub>2"
+          have "x \<notin> \<V>\<^sub>1"
+            using \<open>x \<in> \<V>\<^sub>2\<close> \<open>(\<V> \<union> \<V>\<^sub>1) \<inter> \<V>\<^sub>2 = {}\<close>
+            by auto
+          have "x \<noteq> v"
+            using \<open>x \<in> \<V>\<^sub>2\<close> \<open>v \<notin> (\<V> \<union> \<V>\<^sub>1 \<union> \<V>\<^sub>2)\<close>
+            by auto
+          show ?thesis
+            unfolding pI'_def
+            using \<open>x \<noteq> v\<close> \<open>x \<notin> \<V>\<^sub>1\<close> \<open>x \<in> \<V>\<^sub>2\<close>
+            by simp
+        qed
+
+        show "pI2 x = pI' x"
+          using x_in x_in_preds x_in_\<V>2
+          by auto
+      next
+        show "eval_formula (formula_of_clause_list \<C>\<^sub>2) vI fI pI2"
+          by (simp add: pI2_model)
+      qed
+    qed
+  next
+    show "eval_formula (Pred v ts) vI fI pI' \<longleftrightarrow> eval_formula (And \<phi>\<^sub>1 \<phi>\<^sub>2) vI fI pI"
+      unfolding eval_formula.simps pI'_def
+      using v\<^sub>1_equisat_\<phi>\<^sub>1 v\<^sub>2_equisat_\<phi>\<^sub>2
+      by simp
+  qed
+next
+  case Connective: (Or \<phi>\<^sub>1 \<phi>\<^sub>2)
+
+  obtain v\<^sub>1 ts\<^sub>1 \<C>\<^sub>1 \<V>\<^sub>1 where
+    te_\<phi>1: "tseitin fresh \<V> \<phi>\<^sub>1 = (v\<^sub>1, ts\<^sub>1, \<C>\<^sub>1, \<V>\<^sub>1)"
+    using prod_cases4 by blast
+
+  obtain v\<^sub>2 ts\<^sub>2 \<C>\<^sub>2 \<V>\<^sub>2 where
+    te_\<phi>2: "tseitin fresh (\<V> \<union> \<V>\<^sub>1) \<phi>\<^sub>2 = (v\<^sub>2, ts\<^sub>2, \<C>\<^sub>2, \<V>\<^sub>2)"
+    using prod_cases4 by blast
+
+  define \<C>\<^sub>0 :: "('p \<times> ('v, 'f) fof_term list) literal list list" where
+    "\<C>\<^sub>0 = [
+      [Pos (v, []), Neg (v\<^sub>1, ts\<^sub>1)],
+      [Pos (v, []), Neg (v\<^sub>2, ts\<^sub>2)],
+      [Neg (v, []), Pos (v\<^sub>2, ts\<^sub>2), Pos (v\<^sub>1, ts\<^sub>1)]]"
+
+  have
+    "v = fresh (\<V> \<union> \<V>\<^sub>1 \<union> \<V>\<^sub>2)" and
+    "\<C> = \<C>\<^sub>0 @ \<C>\<^sub>1 @ \<C>\<^sub>2" and
+    "\<V>' = insert v (\<V>\<^sub>1 \<union> \<V>\<^sub>2)"
+    using Connective.prems[simplified, unfolded te_\<phi>1, simplified, unfolded te_\<phi>2, simplified]
+    by (auto simp add: \<C>\<^sub>0_def Let_def)
+
+  obtain pI1 where
+    pI1_extends_pI: "\<forall>x\<in>predicates_of_formula \<phi>\<^sub>1. pI1 x = pI x" and
+    pI1_model: "eval_formula (formula_of_clause_list \<C>\<^sub>1) vI fI pI1" and
+    v\<^sub>1_equisat_\<phi>\<^sub>1: "eval_formula (Pred v\<^sub>1 ts\<^sub>1) vI fI pI1 \<longleftrightarrow> eval_formula \<phi>\<^sub>1 vI fI pI"
+    using Connective.IH(1)[OF _ _ te_\<phi>1] Connective.prems(1,2)
+    by auto
+
+  obtain pI2 where
+    pI2_extends_pI: "\<forall>x\<in>predicates_of_formula \<phi>\<^sub>2. pI2 x = pI x" and
+    pI2_model: "eval_formula (formula_of_clause_list \<C>\<^sub>2) vI fI pI2" and
+    v\<^sub>2_equisat_\<phi>\<^sub>2: "eval_formula (Pred v\<^sub>2 ts\<^sub>2) vI fI pI2 \<longleftrightarrow> eval_formula \<phi>\<^sub>2 vI fI pI"
+    using Connective.IH(2)[OF _ _ te_\<phi>2] te_\<phi>1 Connective.prems(1,2)
+    by (metis (no_types, lifting) Connective.hyps(1)
+        finite_Un formula.simps(208) le_sup_iff
+        sup.coboundedI2 sup_commute
+        tseitin_finite_var_set)
+
+  define pI' :: "'p \<Rightarrow> 'd list \<Rightarrow> bool" where
+    "pI' = (\<lambda>x ds. 
+      if x = v then pI1 v\<^sub>1 (map (\<lambda>t. eval_term t vI fI) ts\<^sub>1) \<or> pI2 v\<^sub>2 (map (\<lambda>t. eval_term t vI fI) ts\<^sub>2) 
+      else (if x \<in> \<V>\<^sub>1 then pI1 x ds 
+      else (if x \<in> \<V>\<^sub>2 then pI2 x ds 
+      else pI x ds)))"
+
+  have "v\<^sub>1 \<in> predicates_of_formula \<phi>\<^sub>1 \<union> \<V>\<^sub>1"
+    using tseitin_generated_var[OF _ te_\<phi>1]
+    by (simp add: Connective.hyps(1))
+
+  have "v\<^sub>2 \<in> predicates_of_formula \<phi>\<^sub>2 \<union> \<V>\<^sub>2"
+    using tseitin_generated_var[OF _ te_\<phi>2]
+    by (simp add: Connective.hyps(2))
+
+  have "\<V> \<inter> \<V>\<^sub>1 = {}"
+    using tseitin_fresh_vars[OF fresh_spec \<open>is_nnf \<phi>\<^sub>1\<close> \<open>finite \<V>\<close> te_\<phi>1]
+    by simp
+
+  have "finite (\<V> \<union> \<V>\<^sub>1)"
+  proof -
+    have "finite \<V>\<^sub>1"
+      using tseitin_finite_var_set[OF \<open>is_nnf \<phi>\<^sub>1\<close> te_\<phi>1]
+      by simp
+    show ?thesis
+      using \<open>finite \<V>\<close> \<open>finite \<V>\<^sub>1\<close>
+      by simp
+  qed
+
+  have "(\<V> \<union> \<V>\<^sub>1) \<inter> \<V>\<^sub>2 = {}"
+    using tseitin_fresh_vars[OF fresh_spec \<open>is_nnf \<phi>\<^sub>2\<close> \<open>finite (\<V> \<union> \<V>\<^sub>1)\<close> te_\<phi>2]
+    by simp
+
+  have "finite (\<V> \<union> \<V>\<^sub>1 \<union> \<V>\<^sub>2)"
+  proof -
+    have "finite \<V>\<^sub>2"
+      using tseitin_finite_var_set[OF \<open>is_nnf \<phi>\<^sub>2\<close> te_\<phi>2]
+      by simp
+    show ?thesis
+      using \<open>finite (\<V> \<union> \<V>\<^sub>1)\<close> \<open>finite \<V>\<^sub>2\<close>
+      by simp
+  qed
+
+  have "v \<in> \<V>'" and "v \<notin> (\<V> \<union> \<V>\<^sub>1 \<union> \<V>\<^sub>2)"
+    unfolding atomize_conj
+  proof (rule conjI)
+    show "v \<in> \<V>'"
+      by (simp add: \<open>\<V>' = insert v (\<V>\<^sub>1 \<union> \<V>\<^sub>2)\<close>)
+  next
+    show "v \<notin> (\<V> \<union> \<V>\<^sub>1 \<union> \<V>\<^sub>2)"
+      unfolding \<open>v = fresh (\<V> \<union> \<V>\<^sub>1 \<union> \<V>\<^sub>2)\<close>
+      using fresh_spec[OF \<open>finite (\<V> \<union> \<V>\<^sub>1 \<union> \<V>\<^sub>2)\<close>]
+      by simp
+  qed
+
+  show ?case
+  proof (intro exI conjI ballI)
+    fix x
+    assume preds: "x \<in> predicates_of_formula (Or \<phi>\<^sub>1 \<phi>\<^sub>2)"
+    have "x \<in> \<V>"
+      using preds Connective.prems(2)
+      by blast
+    have x_ne_v: "x \<noteq> v"
+      using \<open>v = fresh (\<V> \<union> \<V>\<^sub>1 \<union> \<V>\<^sub>2)\<close> \<open>x \<in> \<V>\<close> fresh_spec
+      by (meson Connective.hyps(1,2)
+          Connective.prems(1) UnCI finite_UnI te_\<phi>1
+          te_\<phi>2 tseitin_finite_var_set)
+    have x_ni_\<V>': "x \<in> \<V> \<Longrightarrow> x \<notin> \<V>'"
+      by (metis Connective.hyps(1,2)
+          Connective.prems(1,3) IntI Or empty_iff
+          fresh_spec tseitin_fresh_vars)
+    have x_ni_\<V>1: "x \<notin> \<V>\<^sub>1" and x_ni_\<V>2: "x \<notin> \<V>\<^sub>2"
+      using \<open>\<V>' = insert v (\<V>\<^sub>1 \<union> \<V>\<^sub>2)\<close> \<open>x \<in> \<V>\<close> x_ni_\<V>'
+      by auto
+    show "pI' x = pI x"
+      unfolding pI'_def
+      using x_ne_v x_ni_\<V>1 x_ni_\<V>2
+      by auto  
+  next
+    show "eval_formula (formula_of_clause_list \<C>) vI fI pI'"
+      unfolding \<open>\<C> = \<C>\<^sub>0 @ \<C>\<^sub>1 @ \<C>\<^sub>2\<close> eval_formula_formula_of_clause_list_append_iff
+    proof(intro conjI)
+      have simp1: "formula_of_clause_list \<C>\<^sub>0 = 
+        And (Or (Pred v\<^sub>1 ts\<^sub>1) (Or (Pred v\<^sub>2 ts\<^sub>2) (Or (Not (Pred v [])) F)))
+            (And (Or (Not (Pred v\<^sub>2 ts\<^sub>2)) (Or (Pred v []) F))
+                 (And (Or (Not (Pred v\<^sub>1 ts\<^sub>1)) (Or (Pred v []) F)) T))"
+        unfolding \<C>\<^sub>0_def formula_of_clause_list_def formula_of_clause_def
+        by simp
+
+      have simp2: "eval_formula (formula_of_clause_list \<C>\<^sub>0) vI fI pI'
+        = eval_formula
+          (And (Or (Pred v\<^sub>1 ts\<^sub>1) (Or (Pred v\<^sub>2 ts\<^sub>2) (Not (Pred v []))))
+               (And (Or (Not (Pred v\<^sub>2 ts\<^sub>2)) (Pred v []))
+                    (Or (Not (Pred v\<^sub>1 ts\<^sub>1)) (Pred v [])))) vI fI pI'"
+        unfolding simp1
+        by simp
+
+      have posv: "eval_formula (Pred v []) vI fI pI'
+        = (pI1 v\<^sub>1 (map (\<lambda>t. eval_term t vI fI) ts\<^sub>1) \<or> pI2 v\<^sub>2 (map (\<lambda>t. eval_term t vI fI) ts\<^sub>2))"
+        unfolding pI'_def
+        by simp
+
+      have posv1: "v\<^sub>1 \<in> \<V>\<^sub>1 \<Longrightarrow> 
+        (eval_formula (Pred v\<^sub>1 ts\<^sub>1) vI fI pI' = pI1 v\<^sub>1 (map (\<lambda>t. eval_term t vI fI) ts\<^sub>1))"
+        unfolding eval_formula.simps pI'_def
+        using \<open>v \<notin> (\<V> \<union> \<V>\<^sub>1 \<union> \<V>\<^sub>2)\<close> 
+        by auto
+
+      have posv2: "v\<^sub>2 \<in> \<V>\<^sub>2 \<Longrightarrow> 
+        (eval_formula (Pred v\<^sub>2 ts\<^sub>2) vI fI pI' = pI2 v\<^sub>2 (map (\<lambda>t. eval_term t vI fI) ts\<^sub>2))"
+      proof -
+        assume "v\<^sub>2 \<in> \<V>\<^sub>2"
+        have "v\<^sub>2 \<notin> \<V>" and "v\<^sub>2 \<notin> \<V>\<^sub>1"
+          unfolding atomize_conj
+          using \<open>v\<^sub>2 \<in> \<V>\<^sub>2\<close> \<open>(\<V> \<union> \<V>\<^sub>1) \<inter> \<V>\<^sub>2 = {}\<close> 
+          by auto
+        have "v\<^sub>2 \<noteq> v"
+          using \<open>v\<^sub>2 \<in> \<V>\<^sub>2\<close> \<open>v \<notin> (\<V> \<union> \<V>\<^sub>1 \<union> \<V>\<^sub>2)\<close>
+          by auto
+        show ?thesis
+          unfolding eval_formula.simps pI'_def
+          by (simp add: \<open>v\<^sub>2 \<in> \<V>\<^sub>2\<close> \<open>v\<^sub>2 \<noteq> v\<close> \<open>v\<^sub>2 \<notin> \<V>\<^sub>1\<close>)
+      qed
+
+      have posv1_pred: "v\<^sub>1 \<in> predicates_of_formula \<phi>\<^sub>1 \<Longrightarrow> 
+        (eval_formula (Pred v\<^sub>1 ts\<^sub>1) vI fI pI' = pI v\<^sub>1 (map (\<lambda>t. eval_term t vI fI) ts\<^sub>1))"
+      proof -
+        assume assumption: "v\<^sub>1 \<in> predicates_of_formula \<phi>\<^sub>1"
+        have pred_\<phi>1_in_\<V>: "predicates_of_formula \<phi>\<^sub>1 \<subseteq> \<V>"
+          using Connective.prems(2) 
+          by auto
+        have "v\<^sub>1 \<in> \<V>"
+          using assumption pred_\<phi>1_in_\<V>
+          by auto
+        have "v\<^sub>1 \<notin> \<V>\<^sub>1"
+          using \<open>v\<^sub>1 \<in> \<V>\<close> \<open>\<V> \<inter> \<V>\<^sub>1 = {}\<close>
+          by auto
+        have "v\<^sub>1 \<notin> \<V>\<^sub>2"
+          using \<open>v\<^sub>1 \<in> \<V>\<close> \<open>(\<V> \<union> \<V>\<^sub>1) \<inter> \<V>\<^sub>2 = {}\<close>
+          by auto
+        have "v\<^sub>1 \<noteq> v"
+          using \<open>v\<^sub>1 \<in> \<V>\<close> \<open>v \<notin> (\<V> \<union> \<V>\<^sub>1 \<union> \<V>\<^sub>2)\<close> 
+          by auto
+        show ?thesis
+          unfolding eval_formula.simps pI'_def
+          by (simp add: \<open>v\<^sub>1 \<noteq> v\<close> \<open>v\<^sub>1 \<notin> \<V>\<^sub>1\<close> \<open>v\<^sub>1 \<notin> \<V>\<^sub>2\<close>)
+      qed
+
+      have posv2_pred: "v\<^sub>2 \<in> predicates_of_formula \<phi>\<^sub>2 \<Longrightarrow> 
+        (eval_formula (Pred v\<^sub>2 ts\<^sub>2) vI fI pI' = pI v\<^sub>2 (map (\<lambda>t. eval_term t vI fI) ts\<^sub>2))"
+      proof -
+        assume assumption: "v\<^sub>2 \<in> predicates_of_formula \<phi>\<^sub>2"
+        have pred_\<phi>2_in_\<V>: "predicates_of_formula \<phi>\<^sub>2 \<subseteq> \<V>"
+          using Connective.prems(2)
+          by auto
+        have "v\<^sub>2 \<in> \<V>"
+          using assumption pred_\<phi>2_in_\<V>
+          by auto
+        have "v\<^sub>2 \<notin> \<V>\<^sub>1"
+          using \<open>v\<^sub>2 \<in> \<V>\<close> \<open>\<V> \<inter> \<V>\<^sub>1 = {}\<close>
+          by auto
+        have "v\<^sub>2 \<notin> \<V>\<^sub>2"
+          using \<open>v\<^sub>2 \<in> \<V>\<close> \<open>(\<V> \<union> \<V>\<^sub>1) \<inter> \<V>\<^sub>2 = {}\<close>
+          by auto
+        have "v\<^sub>2 \<noteq> v"
+          using \<open>v\<^sub>2 \<in> \<V>\<close> \<open>v \<notin> (\<V> \<union> \<V>\<^sub>1 \<union> \<V>\<^sub>2)\<close>
+          by auto
+        show ?thesis
+          unfolding eval_formula.simps pI'_def
+          by (simp add: \<open>v\<^sub>2 \<noteq> v\<close> \<open>v\<^sub>2 \<notin> \<V>\<^sub>1\<close> \<open>v\<^sub>2 \<notin> \<V>\<^sub>2\<close>)
+      qed
+
+      consider
+        (A) "v\<^sub>1 \<in> predicates_of_formula \<phi>\<^sub>1 \<and> (v\<^sub>2 \<in> predicates_of_formula \<phi>\<^sub>2)" |
+        (B) "v\<^sub>1 \<in> predicates_of_formula \<phi>\<^sub>1 \<and> (v\<^sub>2 \<in> \<V>\<^sub>2)" |
+        (C) "v\<^sub>1 \<in> \<V>\<^sub>1 \<and> (v\<^sub>2 \<in> predicates_of_formula \<phi>\<^sub>2)" |
+        (D) "v\<^sub>1 \<in> \<V>\<^sub>1 \<and> (v\<^sub>2 \<in> \<V>\<^sub>2)"
+        using
+          \<open>v\<^sub>1 \<in> predicates_of_formula \<phi>\<^sub>1 \<union> \<V>\<^sub>1\<close>
+          \<open>v\<^sub>2 \<in> predicates_of_formula \<phi>\<^sub>2 \<union> \<V>\<^sub>2\<close>
+        by blast
+
+      then show "eval_formula (formula_of_clause_list \<C>\<^sub>0) vI fI pI'"
+      proof cases
+        case A
+        then show ?thesis
+          unfolding simp2
+          using posv posv1_pred posv2_pred pI1_extends_pI pI2_extends_pI
+          by auto
+      next
+        case B
+        then show ?thesis
+          unfolding simp2
+          using posv posv2 posv1_pred pI1_extends_pI
+          by auto
+      next
+        case C
+        then show ?thesis 
+          unfolding simp2
+          using posv posv1 posv2_pred pI2_extends_pI
+          by auto
+      next
+        case D
+        then show ?thesis
+          unfolding simp2
+          using posv posv1 posv2
+          by auto
+      qed
+    next
+      show "eval_formula (formula_of_clause_list \<C>\<^sub>1) vI fI pI'"
+      proof (rule eval_formula_cong_wrt_predicate_evaluation[THEN iffD1, of _ pI1])
+        fix x
+        assume assumption: "x \<in> predicates_of_formula (formula_of_clause_list \<C>\<^sub>1)"
+
+        have ins_v: "insert v\<^sub>1 (predicates_of_formula (formula_of_clause_list \<C>\<^sub>1))
+          = predicates_of_formula \<phi>\<^sub>1 \<union> \<V>\<^sub>1"
+          unfolding predicates_of_formula_of_clause_list
+          unfolding predicates_of_formula_of_clause
+          using tseitin_generated_vars[OF \<open>is_nnf \<phi>\<^sub>1\<close> te_\<phi>1]
+          by simp
+
+        have x_in: "x \<in> predicates_of_formula \<phi>\<^sub>1 \<union> \<V>\<^sub>1"
+          using assumption ins_v
+          by auto
+
+        have x_in_preds: "x \<in> predicates_of_formula \<phi>\<^sub>1 \<Longrightarrow> pI1 x = pI' x" 
+        proof -
+          assume assm: "x \<in> predicates_of_formula \<phi>\<^sub>1"
+          have "x \<in> \<V>"
+          proof -
+            have "predicates_of_formula \<phi>\<^sub>1 \<subseteq> predicates_of_formula (And \<phi>\<^sub>1 \<phi>\<^sub>2)"
+              by simp
+            also have subset: "... \<subseteq> \<V>"
+              using \<open>predicates_of_formula (Or \<phi>\<^sub>1 \<phi>\<^sub>2) \<subseteq> \<V>\<close>
+              by simp
+            show ?thesis
+              using subset assm
+              by auto
+          qed
+          have "x \<notin> \<V>\<^sub>2"
+            using \<open>x \<in> \<V>\<close> \<open>(\<V> \<union> \<V>\<^sub>1) \<inter> \<V>\<^sub>2 = {}\<close>
+            by auto
+          have "x \<noteq> v"
+            using \<open>x \<in> \<V>\<close> \<open>v \<notin> (\<V> \<union> \<V>\<^sub>1 \<union> \<V>\<^sub>2)\<close> 
+            by auto
+          show ?thesis
+            unfolding pI'_def
+            using \<open>x \<noteq> v\<close> \<open>x \<notin> \<V>\<^sub>2\<close> assm pI1_extends_pI 
+            by simp
+        qed
+
+        have x_in_\<V>1: "x \<in> \<V>\<^sub>1 \<Longrightarrow> pI1 x = pI' x"
+        proof -
+          assume "x \<in> \<V>\<^sub>1"
+          have "x \<noteq> v"
+            using \<open>x \<in> \<V>\<^sub>1\<close> \<open>v \<notin> (\<V> \<union> \<V>\<^sub>1 \<union> \<V>\<^sub>2)\<close>
+            by auto
+          show ?thesis
+            unfolding pI'_def
+            using \<open>x \<noteq> v\<close> \<open>x \<in> \<V>\<^sub>1\<close>
+            by simp
+        qed
+
+        show "pI1 x = pI' x"
+          using x_in x_in_preds x_in_\<V>1
+          by blast
+      next
+        show "eval_formula (formula_of_clause_list \<C>\<^sub>1) vI fI pI1"
+          by (simp add: pI1_model)
+      qed
+    next
+      show "eval_formula (formula_of_clause_list \<C>\<^sub>2) vI fI pI'"
+      proof (rule eval_formula_cong_wrt_predicate_evaluation[THEN iffD1, of _ pI2])
+        fix x
+        assume assumption: "x \<in> predicates_of_formula (formula_of_clause_list \<C>\<^sub>2)"
+
+        have ins_v: "insert v\<^sub>2 (predicates_of_formula (formula_of_clause_list \<C>\<^sub>2))
+          = predicates_of_formula \<phi>\<^sub>2 \<union> \<V>\<^sub>2"
+          unfolding predicates_of_formula_of_clause_list
+          unfolding predicates_of_formula_of_clause
+          using tseitin_generated_vars[OF \<open>is_nnf \<phi>\<^sub>2\<close> te_\<phi>2]
+          by simp
+
+        have x_in: "x \<in> predicates_of_formula \<phi>\<^sub>2 \<union> \<V>\<^sub>2"
+          using assumption ins_v
+          by auto
+
+        have x_in_preds: "x \<in> predicates_of_formula \<phi>\<^sub>2 \<Longrightarrow> pI2 x = pI' x" 
+        proof -
+          assume assm: "x \<in> predicates_of_formula \<phi>\<^sub>2"
+          have "x \<in> \<V>"
+          proof -
+            have "predicates_of_formula \<phi>\<^sub>2 \<subseteq> predicates_of_formula (And \<phi>\<^sub>1 \<phi>\<^sub>2)"
+              by simp
+            also have subset: "... \<subseteq> \<V>"
+              using \<open>predicates_of_formula (Or \<phi>\<^sub>1 \<phi>\<^sub>2) \<subseteq> \<V>\<close>
+              by simp
+            show ?thesis
+              using subset assm
+              by auto
+          qed
+          have "x \<notin> \<V>\<^sub>1"
+            using \<open>x \<in> \<V>\<close> \<open>\<V> \<inter> \<V>\<^sub>1 = {}\<close>
+            by auto
+          have "x \<noteq> v"
+            using \<open>x \<in> \<V>\<close> \<open>v \<notin> (\<V> \<union> \<V>\<^sub>1 \<union> \<V>\<^sub>2)\<close> 
+            by auto
+          show ?thesis
+            unfolding pI'_def
+            using \<open>x \<noteq> v\<close> \<open>x \<notin> \<V>\<^sub>1\<close> assm pI2_extends_pI
+            by simp
+        qed
+
+        have x_in_\<V>2: "x \<in> \<V>\<^sub>2 \<Longrightarrow> pI2 x = pI' x"
+        proof -
+          assume "x \<in> \<V>\<^sub>2"
+          have "x \<notin> \<V>\<^sub>1"
+            using \<open>x \<in> \<V>\<^sub>2\<close> \<open>(\<V> \<union> \<V>\<^sub>1) \<inter> \<V>\<^sub>2 = {}\<close>
+            by auto
+          have "x \<noteq> v"
+            using \<open>x \<in> \<V>\<^sub>2\<close> \<open>v \<notin> (\<V> \<union> \<V>\<^sub>1 \<union> \<V>\<^sub>2)\<close>
+            by auto
+          show ?thesis
+            unfolding pI'_def
+            using \<open>x \<noteq> v\<close> \<open>x \<notin> \<V>\<^sub>1\<close> \<open>x \<in> \<V>\<^sub>2\<close>
+            by simp
+        qed
+
+        show "pI2 x = pI' x"
+          using x_in x_in_preds x_in_\<V>2
+          by auto
+      next
+        show "eval_formula (formula_of_clause_list \<C>\<^sub>2) vI fI pI2"
+          by (simp add: pI2_model)
+      qed
+    qed
+  next
+    show "eval_formula (Pred v ts) vI fI pI' \<longleftrightarrow> eval_formula (Or \<phi>\<^sub>1 \<phi>\<^sub>2) vI fI pI"
+      unfolding eval_formula.simps pI'_def
+      using v\<^sub>1_equisat_\<phi>\<^sub>1 v\<^sub>2_equisat_\<phi>\<^sub>2
+      by simp
+  qed
+qed
+
+lemma model_for_tseitin_is_model_for_formula:
+  fixes fresh :: "'p set \<Rightarrow> 'p"
+  assumes fresh_spec: "\<And>\<V>. finite \<V> \<Longrightarrow> fresh \<V> \<notin> \<V>"
+  fixes \<phi> :: "('v, 'f, 'p) formula" and pI :: "'p \<Rightarrow> 'd list \<Rightarrow> bool"
+  assumes "is_nnf \<phi>"
+  assumes "finite \<V>" and "predicates_of_formula \<phi> \<subseteq> \<V>"
+  assumes tseitin: "tseitin fresh \<V> \<phi> = (v, ts, \<C>, \<V>')"
+  assumes eval_te: "eval_formula (And (Pred v ts) (formula_of_clause_list \<C>)) vI fI pI"
+  shows "eval_formula \<phi> vI fI pI"
+  using \<open>is_nnf \<phi>\<close> \<open>finite \<V>\<close> \<open>predicates_of_formula \<phi> \<subseteq> \<V>\<close> tseitin eval_te
+proof (induction \<phi> arbitrary: \<V> v ts \<C> \<V>' rule: is_nnf.induct)
+  case (PosPred p ts\<^sub>p)
+  show ?case
+    using PosPred.prems(3,4)
+    by fastforce
+next
+  case (NegPred p ts\<^sub>p)
+
+  define C\<^sub>1 :: "('p \<times> ('v, 'f) fof_term list) literal list" where
+    "C\<^sub>1 = [Neg (v, []), Neg (p, ts\<^sub>p)]"
+  define C\<^sub>2 :: "('p \<times> ('v, 'f) fof_term list) literal list" where
+    "C\<^sub>2 = [Pos (v, []), Pos (p, ts\<^sub>p)]"
+
+  define \<C>\<^sub>0 :: "('p \<times> ('v, 'f) fof_term list) literal list list" where
+    "\<C>\<^sub>0 = [C\<^sub>1, C\<^sub>2]"
+
+  have "ts = []" and
+       "\<C> = \<C>\<^sub>0"
+    unfolding atomize_conj
+    using NegPred.prems[simplified] \<C>\<^sub>0_def C\<^sub>1_def C\<^sub>2_def
+    by (metis prod.inject)
+
+  have eval_te1: "eval_formula (Pred v ts) vI fI pI"
+    using NegPred.prems(4) 
+    by auto
+
+  have eval_te2: "eval_formula (formula_of_clause_list \<C>) vI fI pI"
+    using NegPred.prems(4) 
+    by auto
+
+  have C_split: "eval_formula (formula_of_clause_list [C\<^sub>1]) vI fI pI
+    \<and> eval_formula (formula_of_clause_list [C\<^sub>2]) vI fI pI"
+    using eval_formula_formula_of_clause_list_append_iff
+    by (metis \<C>\<^sub>0_def \<open>\<C> = \<C>\<^sub>0\<close>
+        append.left_neutral append_Cons
+        eval_te2)
+
+  have cl1: "eval_formula (formula_of_clause_list [C\<^sub>1]) vI fI pI"
+    by (simp add: C_split)
+
+  have cl1_simp: "(formula_of_clause_list [C\<^sub>1])
+    = (And (Or (Not (Pred p ts\<^sub>p)) (Or (Not (Pred v [])) F)) T)"
+    unfolding formula_of_clause_list_def formula_of_clause_def formula_of_literal.simps C\<^sub>1_def
+    by simp
+
+  have final_c1: "eval_formula (And (Or (Not (Pred p ts\<^sub>p)) (Or (Not (Pred v [])) F)) T) vI fI pI"
+    using cl1 cl1_simp
+    by auto
+
+  show ?case
+    using \<open>ts = []\<close> eval_te1 final_c1
+    by auto
+next
+  case Connective: (And \<phi>\<^sub>1 \<phi>\<^sub>2)
+
+  obtain v\<^sub>1 ts\<^sub>1 \<C>\<^sub>1 \<V>\<^sub>1 where
+    te_\<phi>1: "tseitin fresh \<V> \<phi>\<^sub>1 = (v\<^sub>1, ts\<^sub>1, \<C>\<^sub>1, \<V>\<^sub>1)"
+    by (metis prod.exhaust)
+
+  obtain v\<^sub>2 ts\<^sub>2 \<C>\<^sub>2 \<V>\<^sub>2 where
+    te_\<phi>2: "tseitin fresh (\<V> \<union> \<V>\<^sub>1) \<phi>\<^sub>2 = (v\<^sub>2, ts\<^sub>2, \<C>\<^sub>2, \<V>\<^sub>2)"
+    by (metis prod.exhaust)
+
+  define C\<^sub>1 :: "('p \<times> ('v, 'f) fof_term list) literal list" where
+    "C\<^sub>1 = [Neg (v, []), Pos (v\<^sub>1, ts\<^sub>1)]"
+  define C\<^sub>2 :: "('p \<times> ('v, 'f) fof_term list) literal list" where
+    "C\<^sub>2 = [Neg (v, []), Pos (v\<^sub>2, ts\<^sub>2)]"
+  define C\<^sub>3 :: "('p \<times> ('v, 'f) fof_term list) literal list" where
+    "C\<^sub>3 = [Pos (v, []), Neg (v\<^sub>1, ts\<^sub>1), Neg (v\<^sub>2, ts\<^sub>2)]"
+
+  define \<C>\<^sub>0 :: "('p \<times> ('v, 'f) fof_term list) literal list list" where
+    "\<C>\<^sub>0 = [C\<^sub>1, C\<^sub>2, C\<^sub>3]"
+
+  have "ts = []" and
+    "\<C> = \<C>\<^sub>0 @ \<C>\<^sub>1 @ \<C>\<^sub>2"
+    unfolding atomize_conj
+    using Connective.prems[simplified, unfolded te_\<phi>1, simplified, unfolded te_\<phi>2, simplified]
+    by (smt (verit) C\<^sub>1_def C\<^sub>2_def C\<^sub>3_def
+        \<C>\<^sub>0_def append_Cons append_self_conv2
+        old.prod.inject)
+
+  have eval_te1: "eval_formula (Pred v ts) vI fI pI"
+    using Connective.prems(4) 
+    by auto
+
+  have eval_te2: "eval_formula (formula_of_clause_list \<C>) vI fI pI"
+    using Connective.prems(4)
+    by auto
+
+  have C_split: "eval_formula (formula_of_clause_list [C\<^sub>1]) vI fI pI
+    \<and> eval_formula (formula_of_clause_list [C\<^sub>2]) vI fI pI
+    \<and> eval_formula (formula_of_clause_list [C\<^sub>3]) vI fI pI"
+    using eval_formula_formula_of_clause_list_append_iff
+    by (metis \<C>\<^sub>0_def \<open>\<C> = \<C>\<^sub>0 @ \<C>\<^sub>1 @ \<C>\<^sub>2\<close>
+        append.left_neutral append_Cons
+        eval_te2)
+
+  have \<phi>1_true: "eval_formula \<phi>\<^sub>1 vI fI pI"
+  proof -
+    have simp1: "eval_formula (And (formula_of_clause C\<^sub>1) T) vI fI pI"
+      using formula_of_clause_list_def
+      by (metis C_split fold_simps(1,2))
+    have simp2: "formula_of_clause C\<^sub>1 = (Or (Pred v\<^sub>1 ts\<^sub>1) (Or (Not (Pred v ts)) F))"
+      unfolding formula_of_clause_def
+      by (simp add: C\<^sub>1_def \<open>ts = []\<close>)
+    have v1_true: "eval_formula (Pred v\<^sub>1 ts\<^sub>1) vI fI pI"
+      using eval_te1 simp1 simp2
+      by auto
+    show ?thesis
+      using Connective.IH(1)[OF _ _ te_\<phi>1] v1_true
+      by (metis Connective.prems(1,2)
+          \<open>\<C> = \<C>\<^sub>0 @ \<C>\<^sub>1 @ \<C>\<^sub>2\<close>
+          equalityE eval_formula.simps(2)
+          eval_formula_formula_of_clause_list_append_iff
+          eval_te2 formula.simps(207) subset_trans
+          sup.coboundedI1)
+  qed
+
+  have \<phi>2_true: "eval_formula \<phi>\<^sub>2 vI fI pI"
+    proof -
+    have simp1: "eval_formula (And (formula_of_clause C\<^sub>2) T) vI fI pI"
+      using formula_of_clause_list_def
+      by (metis C_split fold_simps(1,2))
+    have simp2: "formula_of_clause C\<^sub>2 = (Or (Pred v\<^sub>2 ts\<^sub>2) (Or (Not (Pred v ts)) F))"
+      unfolding formula_of_clause_def
+      by (simp add: C\<^sub>2_def \<open>ts = []\<close>)
+    have v2_true: "eval_formula (Pred v\<^sub>2 ts\<^sub>2) vI fI pI"
+      using eval_te1 simp1 simp2
+      by auto
+    show ?thesis
+      using Connective.IH(2)[OF _ _ te_\<phi>2] v2_true
+      by (metis Connective.hyps(1)
+          Connective.prems(1,2)
+          \<open>\<C> = \<C>\<^sub>0 @ \<C>\<^sub>1 @ \<C>\<^sub>2\<close>
+          eval_formula.simps(2)
+          eval_formula_formula_of_clause_list_append_iff
+          eval_te2 finite_UnI formula.simps(207)
+          le_supE le_supI1 te_\<phi>1
+          tseitin_finite_var_set)
+  qed
+
+  show ?case
+    by (simp add: \<phi>1_true \<phi>2_true)
+next
+  case Connective: (Or \<phi>\<^sub>1 \<phi>\<^sub>2)
+
+  obtain v\<^sub>1 ts\<^sub>1 \<C>\<^sub>1 \<V>\<^sub>1 where
+    te_\<phi>1: "tseitin fresh \<V> \<phi>\<^sub>1 = (v\<^sub>1, ts\<^sub>1, \<C>\<^sub>1, \<V>\<^sub>1)"
+    by (metis prod.exhaust)
+
+  obtain v\<^sub>2 ts\<^sub>2 \<C>\<^sub>2 \<V>\<^sub>2 where
+    te_\<phi>2: "tseitin fresh (\<V> \<union> \<V>\<^sub>1) \<phi>\<^sub>2 = (v\<^sub>2, ts\<^sub>2, \<C>\<^sub>2, \<V>\<^sub>2)"
+    by (metis prod.exhaust)
+
+  define C\<^sub>1 :: "('p \<times> ('v, 'f) fof_term list) literal list" where
+    "C\<^sub>1 = [Pos (v, []), Neg (v\<^sub>1, ts\<^sub>1)]"
+  define C\<^sub>2 :: "('p \<times> ('v, 'f) fof_term list) literal list" where
+    "C\<^sub>2 = [Pos (v, []), Neg (v\<^sub>2, ts\<^sub>2)]"
+  define C\<^sub>3 :: "('p \<times> ('v, 'f) fof_term list) literal list" where
+    "C\<^sub>3 = [Neg (v, []), Pos (v\<^sub>2, ts\<^sub>2), Pos (v\<^sub>1, ts\<^sub>1)]"
+
+  define \<C>\<^sub>0 :: "('p \<times> ('v, 'f) fof_term list) literal list list" where
+    "\<C>\<^sub>0 = [C\<^sub>1, C\<^sub>2, C\<^sub>3]"
+
+  have "ts = []" and
+    "\<C> = \<C>\<^sub>0 @ \<C>\<^sub>1 @ \<C>\<^sub>2"
+    unfolding atomize_conj
+    using Connective.prems[simplified, unfolded te_\<phi>1, simplified, unfolded te_\<phi>2, simplified]
+    by (smt (verit) C\<^sub>1_def C\<^sub>2_def C\<^sub>3_def
+        \<C>\<^sub>0_def append_Cons append_self_conv2
+        old.prod.inject)
+
+  have eval_te1: "eval_formula (Pred v ts) vI fI pI"
+    using Connective.prems(4) 
+    by auto
+
+  have eval_te2: "eval_formula (formula_of_clause_list \<C>) vI fI pI"
+    using Connective.prems(4)
+    by auto
+
+  have C_split: "eval_formula (formula_of_clause_list [C\<^sub>1]) vI fI pI
+    \<and> eval_formula (formula_of_clause_list [C\<^sub>2]) vI fI pI
+    \<and> eval_formula (formula_of_clause_list [C\<^sub>3]) vI fI pI"
+    using eval_formula_formula_of_clause_list_append_iff
+    by (metis \<C>\<^sub>0_def \<open>\<C> = \<C>\<^sub>0 @ \<C>\<^sub>1 @ \<C>\<^sub>2\<close>
+        append.left_neutral append_Cons
+        eval_te2)
+
+  have simp1: "eval_formula (And (formula_of_clause C\<^sub>3) T) vI fI pI"
+    unfolding atomize_conj
+    using formula_of_clause_list_def
+    by (metis C_split fold_simps(1,2))
+
+  have simp2: "formula_of_clause C\<^sub>3 = Or (Pred v\<^sub>1 ts\<^sub>1) (Or (Pred v\<^sub>2 ts\<^sub>2) (Or (Not (Pred v ts)) F))"
+    unfolding formula_of_clause_def
+    by (simp add: C\<^sub>3_def \<open>ts = []\<close>)
+
+  have v1_or_v2_true: "eval_formula (Pred v\<^sub>1 ts\<^sub>1) vI fI pI \<or> eval_formula (Pred v\<^sub>2 ts\<^sub>2) vI fI pI"
+    using eval_te1 simp1 simp2 
+    by force
+
+  have \<phi>1_or_\<phi>2_true: "eval_formula \<phi>\<^sub>1 vI fI pI \<or> eval_formula \<phi>\<^sub>2 vI fI pI"
+    using Connective.IH(1)[OF _ _ te_\<phi>1] Connective.IH(2)[OF _ _ te_\<phi>2] v1_or_v2_true
+    by (metis Connective.hyps(1)
+        Connective.prems(1,2)
+        \<open>\<C> = \<C>\<^sub>0 @ \<C>\<^sub>1 @ \<C>\<^sub>2\<close>
+        eval_formula.simps(2)
+        eval_formula_formula_of_clause_list_append_iff
+        eval_te2 finite_UnI formula.simps(208)
+        le_supE le_supI1 te_\<phi>1
+        tseitin_finite_var_set)
+
+  show ?case 
+    using \<phi>1_or_\<phi>2_true 
+    by auto
+qed
+
+definition tseitin_expansion where
+  "tseitin_expansion fresh \<phi> =
+    (let (v, ts, \<C>, _) = tseitin fresh (predicates_of_formula \<phi>) \<phi>
+     in And (Pred v ts) (formula_of_clause_list \<C>))"
+
+theorem tseitin_expansion_equisat:
+  fixes fresh :: "'p set \<Rightarrow> 'p"
+  assumes fresh_spec: "\<And>\<V>. finite \<V> \<Longrightarrow> fresh \<V> \<notin> \<V>"
+  fixes \<phi> :: "('v, 'f, 'p) formula"
+  assumes "is_nnf \<phi>"
+  shows "(\<exists>pI. eval_formula \<phi> vI fI pI) \<longleftrightarrow>
+    (\<exists>pI. eval_formula (tseitin_expansion fresh \<phi>) vI fI pI)"
+  (is "?LHS \<longleftrightarrow> ?RHS")
+proof (rule iffI)
+  define \<V> where
+    "\<V> = predicates_of_formula \<phi>"
+
+  have "predicates_of_formula \<phi> = \<V>"
+    by (simp add: \<V>_def)
+
+  have "finite \<V>"
+    unfolding \<V>_def
+    by (simp add: predicates_of_formula_finite)
+
+  have "predicates_of_formula \<phi> \<subseteq> \<V>"
+    unfolding \<V>_def
+    by simp
+
+  obtain v ts \<C> \<V>' where tseitin: "tseitin fresh \<V> \<phi> = (v, ts, \<C>, \<V>')"
+    by (metis prod.exhaust)
+
+  show "?LHS \<Longrightarrow> ?RHS"
+    unfolding tseitin_expansion_def \<open>predicates_of_formula \<phi> = \<V>\<close> tseitin Let_def prod.case
+  proof -
+    assume assumption: "\<exists>pI. eval_formula \<phi> vI fI pI"
+    obtain pI where \<phi>_pI: "eval_formula \<phi> vI fI pI"
+      using assumption 
+      by auto
+    obtain pI' where
+      pI'_model: "eval_formula (formula_of_clause_list \<C>) vI fI pI'" and
+      v_equisat_\<phi>: "eval_formula (Pred v ts) vI fI pI' \<longleftrightarrow> eval_formula \<phi> vI fI pI"
+      using tseitin_spec[OF _ \<open>is_nnf \<phi>\<close> \<open>finite \<V>\<close> \<open>predicates_of_formula \<phi> \<subseteq> \<V>\<close> tseitin]
+      using fresh_spec 
+      by blast
+    have eval_tseitin_\<phi>: "eval_formula (And (Pred v ts) (formula_of_clause_list \<C>)) vI fI pI'"
+      using \<phi>_pI pI'_model v_equisat_\<phi>
+      by auto
+    show "\<exists>pI. eval_formula (And (Pred v ts) (formula_of_clause_list \<C>)) vI fI pI"
+      using eval_tseitin_\<phi> 
+      by auto
+  qed
+  
+  show "?RHS \<Longrightarrow> ?LHS"
+    unfolding tseitin_expansion_def \<open>predicates_of_formula \<phi> = \<V>\<close> tseitin Let_def prod.case
+  proof -
+    assume assumption: "\<exists>pI. eval_formula (And (Pred v ts) (formula_of_clause_list \<C>)) vI fI pI"
+    obtain pI where te_pI: "eval_formula (And (Pred v ts) (formula_of_clause_list \<C>)) vI fI pI"
+      using assumption
+      by auto
+    have eval_\<phi>: "eval_formula \<phi> vI fI pI"
+      using model_for_tseitin_is_model_for_formula
+        [OF _ \<open>is_nnf \<phi>\<close> \<open>finite \<V>\<close> \<open>predicates_of_formula \<phi> \<subseteq> \<V>\<close> tseitin te_pI]
+      by (simp add: fresh_spec)
+    show "?LHS"
+      using eval_\<phi>
+      by auto
+  qed
+qed
+
+(*EXTRAS*)
 (*
-fun tseitin_simp_formula :: "('v, 'f, 'p) formula \<Rightarrow> ('v, 'f, 'p) formula" where
-"tseitin_simp_formula (Pred p []) = Pred p []" |
-"tseitin_simp_formula (And \<phi>1 \<phi>2) = And (tseitin_simp_formula \<phi>1) (tseitin_simp_formula \<phi>2)" |
-"tseitin_simp_formula (Or \<phi>1 \<phi>2) = Or (tseitin_simp_formula \<phi>1) (tseitin_simp_formula \<phi>2)" |
-"tseitin_simp_formula (Not \<phi>) = (case tseitin_simp_formula \<phi> of
-  Pred p [] \<Rightarrow> Not (Pred p []) |
-  Not (Pred p []) \<Rightarrow> Pred p []
-)" |
-"tseitin_simp_formula \<phi> = \<phi>"
+section \<open>Number of Introduced Fresh Variables\<close>
+
+primrec branches :: "('v, 'f, 'p) formula \<Rightarrow> nat" where
+  "branches T = 0" |
+  "branches F = 0" |
+  "branches (Pred _ _) = 0" |
+  "branches (Equal _ _) = 0" |
+  "branches (Not \<phi>) = Suc (branches \<phi>)" |
+  "branches (And \<phi>\<^sub>1 \<phi>\<^sub>2) = Suc (branches \<phi>\<^sub>1 + branches \<phi>\<^sub>2)" |
+  "branches (Or \<phi>\<^sub>1 \<phi>\<^sub>2) = Suc (branches \<phi>\<^sub>1 + branches \<phi>\<^sub>2)" |
+  "branches (Forall _ \<phi>) = Suc (branches \<phi>)" |
+  "branches (Exists _ \<phi>) = Suc (branches \<phi>)"
+
+lemma tseitin_card_vars:
+  fixes fresh :: "'p set \<Rightarrow> 'p"
+  assumes fresh_spec: "\<And>\<V>. finite \<V> \<Longrightarrow> fresh \<V> \<notin> \<V>"
+  fixes \<phi> :: "('v, 'f, 'p) formula"
+  assumes tseitin: "tseitin fresh \<V> \<phi> = (v, ts, \<C>, \<V>')"
+  assumes "finite \<V>" and "is_nnf \<phi>"
+  shows "card \<V>' = branches \<phi>"
+  sorry
+
+theorem tseitin_expansion_card_vars:
+  fixes fresh :: "'p set \<Rightarrow> 'p"
+  assumes fresh_spec: "\<And>\<V>. finite \<V> \<Longrightarrow> fresh \<V> \<notin> \<V>"
+  assumes "is_nnf \<phi>"
+  shows "card (predicates_of_formula (tseitin_expansion fresh \<phi>)) =
+    card (predicates_of_formula \<phi>) + branches \<phi>"
+  sorry
 *)
 
-fun tseitin_equiv_binding :: 
-"('v, 'f, 'p) formula \<Rightarrow> ('v, 'f, 'p) formula \<Rightarrow> ('v, 'f, 'p) formula \<Rightarrow> ('v, 'f, 'p) formula" where
-"tseitin_equiv_binding (Pred _ []) l r = And l r" |
-"tseitin_equiv_binding (Not (Pred _ [])) l r = And l r" |
-"tseitin_equiv_binding (And _ _) l r =
-  (let l' = distribute_formula l;
-       r' = demorg_formula r
-    in And l' r')" |
-"tseitin_equiv_binding (Or _ _) l r =
-  (let r' = demorg_formula r;
-       r'' = distribute_formula r'
-    in And l r'')" |
-"tseitin_equiv_binding _ l r = And l r"
 
-fun tseitin_transform_to_clause :: "('v, 'f, 'p) tseitin_asgnm \<Rightarrow> ('v, 'f, 'p) formula" where
-"tseitin_transform_to_clause (\<tau>, \<phi>) =
-  (let \<tau>_conv = Pred \<tau> [];
-       l = Imp \<tau>_conv \<phi>;
-       r = Imp \<phi> \<tau>_conv;
-       equiv = tseitin_equiv_binding \<phi> l r
-    in simp_formula equiv
-)"
+(*Proved but not used*)
+(**)
+lemma tseitin_fresh_var_in_fresh_var_set:
+  assumes "is_nnf \<phi>"
+  assumes "predicates_of_formula \<phi> \<subseteq> \<V>"
+  assumes tseitin: "tseitin fresh \<V> \<phi> = (v, ts, \<C>, \<V>')"
+  shows "v \<in> (if \<V>' = {} then \<V> else \<V>')"
+  using assms
+proof (induction \<phi>  arbitrary: \<V> v ts \<C> \<V>' rule: is_nnf.induct)
+  case (PosPred p ts\<^sub>p)
 
-fun tseitin_get_head_var :: 
-"('v, 'f, 'p) formula \<Rightarrow> ('v, 'f, 'p) tseitin_asgnm list \<Rightarrow> 'p" where
-"tseitin_get_head_var (Pred p []) [] = p" |
-"tseitin_get_head_var _ as = fst (hd as)"
-
-fun tseitin_get_new_vars :: "('v, 'f, 'p) tseitin_asgnm list \<Rightarrow> 'p set" where
-"tseitin_get_new_vars [] = {}" |
-"tseitin_get_new_vars (a # as) = {fst a} \<union> tseitin_get_new_vars as"
-
-definition tseitin_decompose ::
-"'p fresh \<Rightarrow> 'p set \<Rightarrow> ('v, 'f, 'p) formula \<Rightarrow> 'p \<times> ('v, 'f, 'p) formula list \<times> 'p set" where
-"tseitin_decompose \<xi> \<Sigma> \<phi> = 
-  (let list = tseitin_list \<phi>;
-       list_asgnm = tseitin_list_asgnm \<xi> \<Sigma> list;
-       list_subst = tseitin_list_subst list_asgnm;
-       list_clause = map tseitin_transform_to_clause list_subst;
-       head_var = tseitin_get_head_var \<phi> list_asgnm;
-       new_vars = tseitin_get_new_vars list_asgnm
-    in (head_var, list_clause, new_vars)
-)"
-
-fun tseitin_conjunct_clauses :: 
-"'p \<Rightarrow> ('v, 'f, 'p) formula list \<Rightarrow> ('v, 'f, 'p) formula" where
-"tseitin_conjunct_clauses p [] = (Pred p [])" |
-"tseitin_conjunct_clauses p cls = fold And cls (Pred p [])"
-
-definition tseitin_expansion :: "'p fresh \<Rightarrow> ('v, 'f, 'p) formula \<Rightarrow> ('v, 'f, 'p) formula" where
-"tseitin_expansion \<xi> \<phi> = 
-  (let (\<tau>, \<C>, \<Sigma>') = tseitin_decompose \<xi> (tseitin_occup_var \<phi>) \<phi>
-    in tseitin_conjunct_clauses \<tau> \<C>
-)"
-
-lemma tseitin_Prop_empty_args:
-  fixes fresh :: "'p set \<Rightarrow> 'p"
-  assumes "\<And>\<P>. finite \<P> \<Longrightarrow> fresh \<P> \<notin> \<P>"
-  shows "tseitin_expansion fresh (Pred p []) = Pred p []" 
-proof -
-  have list_asgnm: "tseitin_list_asgnm fresh {p} [] = []"
+  have  "v = p" and
+        "ts = ts\<^sub>p" and
+        "\<C> = []" and
+        "\<V>' = {}"
+    unfolding atomize_conj
+    using PosPred.prems[simplified]
     by simp
-  have to_clause: "map tseitin_transform_to_clause [] = []"
-    by simp
-  have decompose: "tseitin_decompose fresh {p} (Pred p []) = (p, [], {})"
-    unfolding tseitin_decompose_def Let_def tseitin_list.simps list_asgnm
-              tseitin_get_head_var.simps tseitin_list_subst.simps
-              to_clause tseitin_get_new_vars.simps
-    by simp
-  show ?thesis
-    unfolding tseitin_expansion_def tseitin_occup_var.simps decompose Let_def
-    by simp
-qed 
 
-theorem eval_tseitin_equiv_eval:
-  fixes fresh :: "'p set \<Rightarrow> 'p" and \<phi> :: "('v, 'f, 'p) formula"
-  assumes "\<And>\<P>. finite \<P> \<Longrightarrow> fresh \<P> \<notin> \<P>"
-  assumes "is_prop_nnf \<phi>"
-  shows "(\<exists>pI. eval_formula (tseitin_expansion fresh \<phi>) vI fI pI) 
-    \<longleftrightarrow> (\<exists>pI. eval_formula \<phi> vI fI pI)"
-  (is "?LHS \<longleftrightarrow> ?RHS")
-  using \<open>is_prop_nnf \<phi>\<close>
-proof (induction \<phi> rule: is_prop_nnf.induct)
-  case (Prop p)
-  then show ?case
-    by (simp add: assms(1) tseitin_Prop_empty_args)
+  have "p \<in> \<V>"
+    using PosPred.prems(1) 
+    by auto
+
+  show ?case
+    by (simp add: \<open>\<V>' = {}\<close> \<open>p \<in> \<V>\<close> \<open>v = p\<close>)
 next
-  case (NProp p)
-  then show ?case
-    sorry
+  case (NegPred p ts\<^sub>p)
+
+  have "v = fresh \<V>" and
+       "ts = []" and
+       "\<V>' = insert v {}"
+    unfolding atomize_conj
+    using NegPred.prems[simplified]
+    by (metis prod.inject)
+
+  show ?case
+    by (simp add: \<open>\<V>' = {v}\<close>)
 next
-  case (And f1 f2)
-  then show ?case
-    sorry
+  case (And \<phi>\<^sub>1 \<phi>\<^sub>2)
+
+  obtain v\<^sub>1 ts\<^sub>1 \<C>\<^sub>1 \<V>\<^sub>1 where
+    te_\<phi>1: "tseitin fresh \<V> \<phi>\<^sub>1 = (v\<^sub>1, ts\<^sub>1, \<C>\<^sub>1, \<V>\<^sub>1)"
+    using prod_cases4 
+    by blast
+
+  obtain v\<^sub>2 ts\<^sub>2 \<C>\<^sub>2 \<V>\<^sub>2 where
+    te_\<phi>2: "tseitin fresh (\<V> \<union> \<V>\<^sub>1) \<phi>\<^sub>2 = (v\<^sub>2, ts\<^sub>2, \<C>\<^sub>2, \<V>\<^sub>2)"
+    using prod_cases4 
+    by blast
+
+  have
+    "v = fresh (\<V> \<union> \<V>\<^sub>1 \<union> \<V>\<^sub>2)" and
+    \<V>'_def: "\<V>' = insert v (\<V>\<^sub>1 \<union> \<V>\<^sub>2)"
+    unfolding atomize_conj
+    using And.prems[simplified, unfolded te_\<phi>1, simplified, unfolded te_\<phi>2, simplified]
+    by (metis Pair_inject)
+
+  show ?case
+    by (simp add: \<V>'_def)
 next
-  case (Or f1 f2)
-  then show ?case
-    sorry
+  case (Or \<phi>\<^sub>1 \<phi>\<^sub>2)
+
+  obtain v\<^sub>1 ts\<^sub>1 \<C>\<^sub>1 \<V>\<^sub>1 where
+    te_\<phi>1: "tseitin fresh \<V> \<phi>\<^sub>1 = (v\<^sub>1, ts\<^sub>1, \<C>\<^sub>1, \<V>\<^sub>1)"
+    using prod_cases4 
+    by blast
+
+  obtain v\<^sub>2 ts\<^sub>2 \<C>\<^sub>2 \<V>\<^sub>2 where
+    te_\<phi>2: "tseitin fresh (\<V> \<union> \<V>\<^sub>1) \<phi>\<^sub>2 = (v\<^sub>2, ts\<^sub>2, \<C>\<^sub>2, \<V>\<^sub>2)"
+    using prod_cases4 
+    by blast
+
+  have
+    "v = fresh (\<V> \<union> \<V>\<^sub>1 \<union> \<V>\<^sub>2)" and
+    \<V>'_def: "\<V>' = insert v (\<V>\<^sub>1 \<union> \<V>\<^sub>2)"
+    unfolding atomize_conj
+    using Or.prems[simplified, unfolded te_\<phi>1, simplified, unfolded te_\<phi>2, simplified]
+    by (metis Pair_inject)
+
+  show ?case
+    by (simp add: \<V>'_def)
 qed
 
 end
