FOF_Tseitin_Initial.thy
@@ -1,0 +1,198 @@
+theory FOF_Tseitin_Initial
+  imports Main FOF_Base FOF_Simplify
+begin
+
+inductive is_prop :: "('v, 'f, 'p) formula \<Rightarrow> bool" where
+Prop: "is_prop (Pred p [])" |
+And: "is_prop f1 \<Longrightarrow> is_prop f2 \<Longrightarrow> is_prop (And f1 f2)" |
+Or: "is_prop f1 \<Longrightarrow> is_prop f2 \<Longrightarrow> is_prop (Or f1 f2)" |
+Not: "is_prop f \<Longrightarrow> is_prop (Not f)"
+
+inductive is_prop_literal :: "('v, 'f, 'p) formula \<Rightarrow> bool" where
+Prop: "is_prop_literal (Pred p [])" |
+NProp: "is_prop_literal (Not (Pred p []))"
+
+inductive is_prop_nnf :: "('v, 'f, 'p) formula \<Rightarrow> bool" where
+Prop: "is_prop_nnf (Pred p [])" |
+NProp: "is_prop_nnf (Not (Pred p []))" |
+And: "is_prop_nnf f1 \<Longrightarrow> is_prop_nnf f2 \<Longrightarrow> is_prop_nnf (And f1 f2)" |
+Or: "is_prop_nnf f1 \<Longrightarrow> is_prop_nnf f2 \<Longrightarrow> is_prop_nnf (Or f1 f2)"
+
+inductive is_prop_clause :: "('v, 'f, 'p) formula \<Rightarrow> bool" where
+Literal: "is_prop_literal f \<Longrightarrow> is_prop_clause f" |
+Or: "is_prop_literal f1 \<Longrightarrow> is_prop_literal f2 \<Longrightarrow> is_prop_clause (Or f1 f2)"
+
+inductive is_cnf :: "('v, 'f, 'p) formula \<Rightarrow> bool" where
+Literal: "is_prop_literal f \<Longrightarrow> is_cnf f" |
+And: "is_prop_clause f1 \<Longrightarrow> is_prop_clause f2 \<Longrightarrow> is_cnf (And f1 f2)" 
+
+type_synonym 'p fresh = "'p set \<Rightarrow> 'p"
+type_synonym ('v, 'f, 'p) tseitin_asgnm = "'p \<times> ('v, 'f, 'p) formula"
+
+fun tseitin_occup_var :: "('v, 'f, 'p) formula \<Rightarrow> 'p set" where
+"tseitin_occup_var (Pred p []) = {p}" |
+"tseitin_occup_var (Not (Pred p [])) = {p}" |
+"tseitin_occup_var (And f1 f2) = tseitin_occup_var f1 \<union> tseitin_occup_var f2" |
+"tseitin_occup_var (Or f1 f2) = tseitin_occup_var f1 \<union> tseitin_occup_var f2" |
+"tseitin_occup_var _ = {}"
+
+fun tseitin_list :: "('v, 'f, 'p) formula \<Rightarrow> ('v, 'f, 'p) formula list" where
+"tseitin_list (Pred p []) = []" |
+"tseitin_list (Not (Pred p [])) = [Not (Pred p [])]" |
+"tseitin_list (And f1 f2) = [And f1 f2] @ tseitin_list f1 @ tseitin_list f2" |
+"tseitin_list (Or f1 f2) = [Or f1 f2] @ tseitin_list f1 @ tseitin_list f2" |
+"tseitin_list _ = []"
+
+definition tseitin_fresh_var :: "'p fresh \<Rightarrow> 'p set \<Rightarrow> 'p \<times> 'p set" where
+"tseitin_fresh_var \<xi> \<Sigma> = (let \<tau> = \<xi> \<Sigma> in (\<tau>, \<Sigma> \<union> {\<tau>}))"
+
+fun tseitin_list_asgnm :: 
+"'p fresh \<Rightarrow> 'p set \<Rightarrow> ('v, 'f, 'p) formula list \<Rightarrow> ('v, 'f, 'p) tseitin_asgnm list" where
+"tseitin_list_asgnm \<xi> \<Sigma> [] = []" |
+"tseitin_list_asgnm \<xi> \<Sigma> (f # fs) = 
+  (let fresh_var = tseitin_fresh_var \<xi> \<Sigma>;
+       assign_var = ((fst fresh_var), f)
+    in assign_var # tseitin_list_asgnm \<xi> (snd fresh_var) fs)"
+
+fun tseitin_subst_formula ::
+"('v, 'f, 'p) formula \<Rightarrow> ('v, 'f, 'p) tseitin_asgnm list \<Rightarrow> ('v, 'f, 'p) formula" where
+"tseitin_subst_formula f [] = f" |
+"tseitin_subst_formula f (a # as) = 
+  (if (f = snd a) 
+   then Pred (fst a) []
+   else tseitin_subst_formula f as)"
+
+fun tseitin_subst_subformula :: 
+"('v, 'f, 'p) formula \<Rightarrow> ('v, 'f, 'p) tseitin_asgnm list \<Rightarrow> ('v, 'f, 'p) formula" where
+"tseitin_subst_subformula f [] = f" |
+"tseitin_subst_subformula (Pred p []) _ = Pred p []" |
+"tseitin_subst_subformula (Not (Pred p [])) _ = Not (Pred p [])" |
+"tseitin_subst_subformula (And f1 f2) as = 
+  (let f1_subst = tseitin_subst_formula f1 as;
+       f2_subst = tseitin_subst_formula f2 as
+    in And f1_subst f2_subst)" |
+"tseitin_subst_subformula (Or f1 f2) as =
+  (let f1_subst = tseitin_subst_formula f1 as;
+       f2_subst = tseitin_subst_formula f2 as
+    in Or f1_subst f2_subst)" |
+"tseitin_subst_subformula f _ = f"
+
+fun tseitin_list_subst :: "('v, 'f, 'p) tseitin_asgnm list \<Rightarrow> ('v, 'f, 'p) tseitin_asgnm list" where
+"tseitin_list_subst [] = []" |
+"tseitin_list_subst ((\<tau>, f) # as) =
+  (let f' = tseitin_subst_subformula f as
+    in (\<tau>, f') # tseitin_list_subst as)"
+
+(*
+fun tseitin_simp_formula :: "('v, 'f, 'p) formula \<Rightarrow> ('v, 'f, 'p) formula" where
+"tseitin_simp_formula (Pred p []) = Pred p []" |
+"tseitin_simp_formula (And \<phi>1 \<phi>2) = And (tseitin_simp_formula \<phi>1) (tseitin_simp_formula \<phi>2)" |
+"tseitin_simp_formula (Or \<phi>1 \<phi>2) = Or (tseitin_simp_formula \<phi>1) (tseitin_simp_formula \<phi>2)" |
+"tseitin_simp_formula (Not \<phi>) = (case tseitin_simp_formula \<phi> of
+  Pred p [] \<Rightarrow> Not (Pred p []) |
+  Not (Pred p []) \<Rightarrow> Pred p []
+)" |
+"tseitin_simp_formula \<phi> = \<phi>"
+*)
+
+fun tseitin_equiv_binding :: 
+"('v, 'f, 'p) formula \<Rightarrow> ('v, 'f, 'p) formula \<Rightarrow> ('v, 'f, 'p) formula \<Rightarrow> ('v, 'f, 'p) formula" where
+"tseitin_equiv_binding (Pred _ []) l r = And l r" |
+"tseitin_equiv_binding (Not (Pred _ [])) l r = And l r" |
+"tseitin_equiv_binding (And _ _) l r =
+  (let l' = distribute_formula l;
+       r' = demorg_formula r
+    in And l' r')" |
+"tseitin_equiv_binding (Or _ _) l r =
+  (let r' = demorg_formula r;
+       r'' = distribute_formula r'
+    in And l r'')" |
+"tseitin_equiv_binding _ l r = And l r"
+
+fun tseitin_transform_to_clause :: "('v, 'f, 'p) tseitin_asgnm \<Rightarrow> ('v, 'f, 'p) formula" where
+"tseitin_transform_to_clause (\<tau>, \<phi>) =
+  (let \<tau>_conv = Pred \<tau> [];
+       l = Imp \<tau>_conv \<phi>;
+       r = Imp \<phi> \<tau>_conv;
+       equiv = tseitin_equiv_binding \<phi> l r
+    in simp_formula equiv
+)"
+
+fun tseitin_get_head_var :: 
+"('v, 'f, 'p) formula \<Rightarrow> ('v, 'f, 'p) tseitin_asgnm list \<Rightarrow> 'p" where
+"tseitin_get_head_var (Pred p []) [] = p" |
+"tseitin_get_head_var _ as = fst (hd as)"
+
+fun tseitin_get_new_vars :: "('v, 'f, 'p) tseitin_asgnm list \<Rightarrow> 'p set" where
+"tseitin_get_new_vars [] = {}" |
+"tseitin_get_new_vars (a # as) = {fst a} \<union> tseitin_get_new_vars as"
+
+definition tseitin_decompose ::
+"'p fresh \<Rightarrow> 'p set \<Rightarrow> ('v, 'f, 'p) formula \<Rightarrow> 'p \<times> ('v, 'f, 'p) formula list \<times> 'p set" where
+"tseitin_decompose \<xi> \<Sigma> \<phi> = 
+  (let list = tseitin_list \<phi>;
+       list_asgnm = tseitin_list_asgnm \<xi> \<Sigma> list;
+       list_subst = tseitin_list_subst list_asgnm;
+       list_clause = map tseitin_transform_to_clause list_subst;
+       head_var = tseitin_get_head_var \<phi> list_asgnm;
+       new_vars = tseitin_get_new_vars list_asgnm
+    in (head_var, list_clause, new_vars)
+)"
+
+fun tseitin_conjunct_clauses :: 
+"'p \<Rightarrow> ('v, 'f, 'p) formula list \<Rightarrow> ('v, 'f, 'p) formula" where
+"tseitin_conjunct_clauses p [] = (Pred p [])" |
+"tseitin_conjunct_clauses p cls = fold And cls (Pred p [])"
+
+definition tseitin_expansion :: "'p fresh \<Rightarrow> ('v, 'f, 'p) formula \<Rightarrow> ('v, 'f, 'p) formula" where
+"tseitin_expansion \<xi> \<phi> = 
+  (let (\<tau>, \<C>, \<Sigma>') = tseitin_decompose \<xi> (tseitin_occup_var \<phi>) \<phi>
+    in tseitin_conjunct_clauses \<tau> \<C>
+)"
+
+lemma tseitin_Prop_empty_args:
+  fixes fresh :: "'p set \<Rightarrow> 'p"
+  assumes "\<And>\<P>. finite \<P> \<Longrightarrow> fresh \<P> \<notin> \<P>"
+  shows "tseitin_expansion fresh (Pred p []) = Pred p []" 
+proof -
+  have list_asgnm: "tseitin_list_asgnm fresh {p} [] = []"
+    by simp
+  have to_clause: "map tseitin_transform_to_clause [] = []"
+    by simp
+  have decompose: "tseitin_decompose fresh {p} (Pred p []) = (p, [], {})"
+    unfolding tseitin_decompose_def Let_def tseitin_list.simps list_asgnm
+              tseitin_get_head_var.simps tseitin_list_subst.simps
+              to_clause tseitin_get_new_vars.simps
+    by simp
+  show ?thesis
+    unfolding tseitin_expansion_def tseitin_occup_var.simps decompose Let_def
+    by simp
+qed 
+
+theorem eval_tseitin_equiv_eval:
+  fixes fresh :: "'p set \<Rightarrow> 'p" and \<phi> :: "('v, 'f, 'p) formula"
+  assumes "\<And>\<P>. finite \<P> \<Longrightarrow> fresh \<P> \<notin> \<P>"
+  assumes "is_prop_nnf \<phi>"
+  shows "(\<exists>pI. eval_formula (tseitin_expansion fresh \<phi>) vI fI pI) 
+    \<longleftrightarrow> (\<exists>pI. eval_formula \<phi> vI fI pI)"
+  (is "?LHS \<longleftrightarrow> ?RHS")
+  using \<open>is_prop_nnf \<phi>\<close>
+proof (induction \<phi> rule: is_prop_nnf.induct)
+  case (Prop p)
+  then show ?case
+    by (simp add: assms(1) tseitin_Prop_empty_args)
+next
+  case (NProp p)
+  then show ?case
+    sorry
+next
+  case (And f1 f2)
+  then show ?case
+    sorry
+next
+  case (Or f1 f2)
+  then show ?case
+    sorry
+qed
+
+end
